@prefix : <http://w3id.org/rsp/vocals-sd#> .
@prefix dc: <http://purl.org/dc/elements/1.1/> .
@prefix sd: <http://www.w3.org/ns/sparql-service-description#> .
@prefix owl: <http://www.w3.org/2002/07/owl#> .
@prefix rdf: <http://www.w3.org/1999/02/22-rdf-syntax-ns#> .
@prefix xml: <http://www.w3.org/XML/1998/namespace> .
@prefix xsd: <http://www.w3.org/2001/XMLSchema#> .
@prefix frmt: <http://www.w3.org/ns/formats/> .
@prefix rdfs: <http://www.w3.org/2000/01/rdf-schema#> .
@prefix time: <http://www.w3.org/2006/time#> .
@prefix vann: <http://purl.org/vocab/vann/> .
@prefix vprov: <http://w3id.org/rsp/vocals-prov#> .
@prefix vocals: <http://w3id.org/rsp/vocals#> .
@prefix dcterms: <http://purl.org/dc/terms/> .
@prefix vocals-sd: <http://w3id.org/rsp/vocals-sd#> .
@base <http://w3id.org/rsp/vocals-sd#> .

<http://w3id.org/rsp/vocals-sd#> rdf:type owl:Ontology ;
                                  owl:versionIRI <http://w3id.org/rsp/vocals-sd> ;
                                  dc:publisher <http://aislab.hevs.ch/> ;
                                  rdfs:comment "Esta ontología has sido diseñada para representar servicios que proveen o manipulan Streams de datos en RDF, así como los endpoints a través de los cuales se puede acceder a los datos de estos streams;  y los meta datos correspondientes."@es ;
                                  dc:creator <https://w3id.org/people/rictomm> ;
                                  dcterms:modified "2017-12-30"^^xsd:date ;
                                  dcterms:title "VoCaLS: ontologie de representation de services pour données et metadonnées de streams RDF"@fr ;
                                  dc:creator <http://w3id.org/people/jpcik/me> ;
                                  dcterms:rights "Copyright © 2017 Politecnico di Milano & HES-SO Valais-Wallis"^^xsd:string ;
                                  dcterms:description "Cette ontologie a été conçue pour representer des services qui genèrent ou consomment données et meta-données de streams RDF, ainsi que leurs points d'accès."@fr ;
                                  rdfs:comment "Cette ontologie a été conçue pour representer des services qui genèrent ou consomment données et meta-données de streams RDF, ainsi que leurs points d'accès."@fr ;
                                  dcterms:title "VoCaLS-SD: Vocabulario y catálogo para Streams enlazados, módulo de descripción de servicios"@es ;
                                  dcterms:license <https://creativecommons.org/licenses/by/4.0/> ;
                                  dcterms:publisher <http://w3id.org/hes-so/aislab> ;
                                  vann:preferredNamespacePrefix "vocals-sd" ;
                                  dcterms:created "2017-12-23T13:00:00"^^xsd:dateTime ;
                                  dcterms:issued "2017-12-29"^^xsd:date ;
                                  dc:creator <http://w3id.org/people/ysedira> ;
                                  rdfs:comment "This ontology aims to model Services for publishing and consuming RDF streams, their metadata, and access endpoints for publishing and consuming these streams"@en ;
                                  owl:versionInfo "0.1.1"^^xsd:string ;
                                  dcterms:description "Esta ontología has sido diseñada para representar servicios que proveen o manipulan Streams de datos en RDF, así como los endpoints a través de los cuales se puede acceder a los datos de estos streams;  y los meta datos correspondientes."@es ;
                                  dcterms:title "VoCaLS-SD: A Vocabulary and Catalog for Linked Streams, Service Description Module"@en ;
                                  dcterms:description "This ontology aims to model Services for publishing and consuming RDF streams, their metadata, and access endpoints for publishing and consuming these streams"@en ;
                                  vann:preferredNamespaceUri "http://w3id.org/rsp/vocals-sd#" .

#################################################################
#    Annotation properties
#################################################################

###  http://w3id.org/rsp/vocals-sd#name
vocals-sd:name rdf:type owl:AnnotationProperty ;
               rdfs:comment "Relates a named time varying graph to the name by which it may be referenced in a FROM/FROM NAMED clause. The object of the name property is an IRI." ;
               rdfs:domain vocals-sd:TimeVaryingGraph .


#################################################################
#    Object Properties
#################################################################

###  http://w3id.org/rsp/vocals-sd#availableGraph
vocals-sd:availableGraph rdf:type owl:ObjectProperty ;
                         rdfs:domain vocals-sd:RDFStreamService ;
                         rdfs:range vocals-sd:TimeVaryingGraph ;
                         rdfs:comment "Relates an instance of RDFStreamService to the time varying graphs available by the RDFStreamService."@en ;
                         rdfs:label "availableGraph"@en .


###  http://w3id.org/rsp/vocals-sd#availableStream
vocals-sd:availableStream rdf:type owl:ObjectProperty ;
                          rdfs:subPropertyOf owl:topObjectProperty ;
                          rdfs:domain vocals-sd:RDFStreamService ;
                          rdfs:range vocals:RDFStream ;
                          rdfs:comment "Relates an RDFStreamService with the RDF streams available in the service"@en ;
                          rdfs:label "availableStream"@en .


###  http://w3id.org/rsp/vocals-sd#defaultGraph
vocals-sd:defaultGraph rdf:type owl:ObjectProperty ;
                       rdfs:domain vocals-sd:StreamingDataset ;
                       rdfs:range vocals-sd:TimeVaryingGraph ;
                       rdfs:comment "Relates an instance of a Streaming Data Set to the description of its default graph."@en ;
                       rdfs:label "defaultGraph"@en .


###  http://w3id.org/rsp/vocals-sd#defaultStreamingDataset
vocals-sd:defaultStreamingDataset rdf:type owl:ObjectProperty ;
                                  rdfs:domain vocals-sd:RDFStreamService ;
                                  rdfs:range vocals-sd:StreamingDataset ;
                                  rdfs:comment "Relates an instance of an RDFStreamService to a description of the default Streaming Dataset available when no explicit dataset is specified."@en ;
                                  rdfs:label "defaultStreamingDataset"@en .


###  http://w3id.org/rsp/vocals-sd#describedBy
vocals-sd:describedBy rdf:type owl:ObjectProperty ;
                      rdfs:domain vocals:RDFStream ;
                      rdfs:range vocals-sd:CatalogService ;
                      rdfs:comment "Points to an instance of a CatalogingService that describes a certain RDFStream."@en ;
                      rdfs:label "describedBy"@en .


###  http://w3id.org/rsp/vocals-sd#endedAt
vocals-sd:endedAt rdf:type owl:ObjectProperty ;
                  rdfs:domain vocals-sd:Window ;
                  rdfs:range time:Instant ;
                  rdfs:label "endedAt"@en ;
                  rdfs:comment "Relates a window and the time instant when it ended"@en .


###  http://w3id.org/rsp/vocals-sd#graph
vocals-sd:graph rdf:type owl:ObjectProperty ;
                rdfs:range vocals-sd:TimeVaryingGraph ;
                rdfs:comment "Relates a named time varying graph to its graph description." ;
                rdfs:label "graph"@en .


###  http://w3id.org/rsp/vocals-sd#hasFeature
vocals-sd:hasFeature rdf:type owl:ObjectProperty ;
                     rdfs:domain vocals-sd:RDFStreamService ;
                     rdfs:range vocals-sd:RDFStreamingFeature ;
                     rdfs:comment "Relates an RDF Stream Service to an available RDF Streaming Feature. This relationship describe the features that the service provides."@en ;
                     rdfs:label "hasFeature"@en .


###  http://w3id.org/rsp/vocals-sd#namedTimeVaryingGraph
vocals-sd:namedTimeVaryingGraph rdf:type owl:ObjectProperty ;
                                rdfs:domain vocals-sd:StreamingDataset ;
                                rdfs:range vocals-sd:TimeVaryingGraph ;
                                rdfs:comment "Relates an instance of StreamingDataset to the description of one of its named time varying graphs. The description of such a named time varying graph MUST include the name property."@en ;
                                rdfs:label "namedTimeVaryingGraph"@en .


###  http://w3id.org/rsp/vocals-sd#publishedBy
vocals-sd:publishedBy rdf:type owl:ObjectProperty ;
                      rdfs:domain vocals:RDFStream ;
                      rdfs:range vocals-sd:PublishingService ;
                      rdfs:comment "Points to an instance of PublishingService that publishs a certain (or certains) RDFStream."@en ;
                      rdfs:label "publishedBy"@en .


###  http://w3id.org/rsp/vocals-sd#registerdTask
vocals-sd:registerdTask rdf:type owl:ObjectProperty ;
                        rdfs:domain vocals-sd:RDFStreamService ;
                        rdfs:comment "Relates an instance of RDFStreamService with instances of running tasks, e.g. RSP-QL Query, other RDF stream processing tasks"@en ;
                        rdfs:label "registerdTask"@en .


###  http://w3id.org/rsp/vocals-sd#registeredBy
vocals-sd:registeredBy rdf:type owl:ObjectProperty ;
                       rdfs:domain vocals:RDFStream ;
                       rdfs:range vocals-sd:ProcessingService ;
                       rdfs:comment "Points to an instance of ProcessingService that registers/ processes a certain RDFStream."@en ;
                       rdfs:label "registeredBy"@en .


###  http://w3id.org/rsp/vocals-sd#registeredStreams
vocals-sd:registeredStreams rdf:type owl:ObjectProperty ;
                            rdfs:domain vocals-sd:RDFStreamService ;
                            rdfs:range vocals:RDFStream ;
                            rdfs:comment "Relates an instance of RDFStreamService to the Stream(s) registered on it."@en ;
                            rdfs:label "registeredStream"@en .


###  http://w3id.org/rsp/vocals-sd#resultFormat
vocals-sd:resultFormat rdf:type owl:ObjectProperty ;
                       rdfs:domain vocals-sd:RDFStreamService ;
                       rdfs:range frmt:Format ;
                       rdfs:comment "Relates an instance of RDFStreamService to a format that is supported for serializing streaming results."@en ;
                       rdfs:label "resultFormat"@en .


###  http://w3id.org/rsp/vocals-sd#rspEndpoint
vocals-sd:rspEndpoint rdf:type owl:ObjectProperty ;
                      rdfs:domain vocals-sd:RDFStreamService ;
                      rdfs:comment "The RSP-QL endpoint of an vocals:RSPService that implements the RSP-QL Protocol service. The object of the rspEndpoint property is an IRI."@en ;
                      rdfs:label "rspEndpoint"@en .


###  http://w3id.org/rsp/vocals-sd#startedAt
vocals-sd:startedAt rdf:type owl:ObjectProperty ;
                    rdfs:domain vocals-sd:Window ;
                    rdfs:range time:Instant ;
                    rdfs:comment "Relates a window and the time instant when it started"@en ;
                    rdfs:label "startedAt"@en .


#################################################################
#    Classes
#################################################################

###  http://w3id.org/rsp/vocals#RDFStream
vocals:RDFStream rdf:type owl:Class .


###  http://w3id.org/rsp/vocals-sd#CatalogService
vocals-sd:CatalogService rdf:type owl:Class ;
                         rdfs:subClassOf vocals-sd:RDFStreamService ;
                         rdfs:comment "An CatalogService is a service providing access to stream descriptions. (e.g. SPARQL endpoint, RDF filse with stream descriptions, etc.)"@en ;
                         rdfs:label "CatalogService"@en ;
                         rdfs:seeAlso "vocals:StreamDescriptor" .


###  http://w3id.org/rsp/vocals-sd#Operation
vocals-sd:Operation rdf:type owl:Class ;
                    rdfs:subClassOf vocals-sd:RDFStreamingFeature ;
                    rdfs:comment "An operation represents an available action/function that can be performed by an RDF Stream Service. An operation may ingest stream items or static data items, and output either of them."@en ;
                    rdfs:label "Operation"@en ;
                    rdfs:seeAlso vocals-sd:RDFStreamService .


###  http://w3id.org/rsp/vocals-sd#PhysicalWindow
vocals-sd:PhysicalWindow rdf:type owl:Class ;
                         rdfs:subClassOf vocals-sd:Window ;
                         rdfs:comment "A PhysicalWindow is a Window defined by an interval size (in units of RDF elements), e.g. a window of n RDF elements."@en ;
                         rdfs:label "PhysicalWindow"@en ;
                         rdfs:seeAlso vocals-sd:Window .


###  http://w3id.org/rsp/vocals-sd#ProcessingService
vocals-sd:ProcessingService rdf:type owl:Class ;
                            rdfs:subClassOf vocals-sd:RDFStreamService ;
                            rdfs:comment "A ProcessingService represents an RDF stream service that provides processing features over RDF streams. Processing refers to any kind of transformation on streaming data, i.e., querying, reasoning, filtering, etc."@en ;
                            rdfs:label "ProcessingService"@en .


###  http://w3id.org/rsp/vocals-sd#PublishingService
vocals-sd:PublishingService rdf:type owl:Class ;
                            rdfs:subClassOf vocals-sd:RDFStreamService ;
                            rdfs:comment "A PublishingService represents an RDF stream service for publishing purposes. Publishing can to be interpreted as Linked Data publishing, where possible, but it may support other types of RDF stream publishing mechanisms as well."@en ;
                            rdfs:label "PublishingService"@en .


###  http://w3id.org/rsp/vocals-sd#QueryModel
vocals-sd:QueryModel rdf:type owl:Class ;
                     rdfs:subClassOf vocals-sd:RDFStreamingFeature ;
                     rdfs:comment "The query model is the type of queries that an RSP enginer can evaluate and answer." .


###  http://w3id.org/rsp/vocals-sd#R2ROperation
vocals-sd:R2ROperation rdf:type owl:Class ;
                       rdfs:subClassOf vocals-sd:Operation ;
                       owl:disjointWith vocals-sd:R2SOperation ,
                                        vocals-sd:S2ROperation ,
                                        vocals-sd:S2SOperation ;
                       rdfs:comment "An R2ROperation represents a realtion-to-relation operation that an RDF Stream Service can perform, such as filtering, aggregation, projection, join, etc. It takes as input a relation (e.g. RDF data mappings) and outputs also a relation (e.g. RDF data mappings)."@en ;
                       rdfs:isDefinedBy "Dell'Aglio, Daniele, et al. \"RSP-QL semantics: a unifying query model to explain heterogeneity of RDF stream processing systems.\" International Journal on Semantic Web and Information Systems (IJSWIS) 10.4 (2014): 17-44." ;
                       rdfs:label "R2ROperation"@en .


###  http://w3id.org/rsp/vocals-sd#R2SOperation
vocals-sd:R2SOperation rdf:type owl:Class ;
                       rdfs:subClassOf vocals-sd:Operation ;
                       rdfs:comment "An R2SOperation represents a realtion-to-stream operation that an RDF Stream Service can perform. It takes as input a relation (e.g. RDF data mappings), and ouputs RDF Stream elements, e.g. for instance an operation that replays a static dataset as a stream, or an Istream, Rstream or Dstream operation."@en ;
                       rdfs:isDefinedBy "Dell'Aglio, Daniele, et al. \"RSP-QL semantics: a unifying query model to explain heterogeneity of RDF stream processing systems.\" International Journal on Semantic Web and Information Systems (IJSWIS) 10.4 (2014): 17-44." ;
                       rdfs:label "R2SOperation"@en .


###  http://w3id.org/rsp/vocals-sd#RDFStreamService
vocals-sd:RDFStreamService rdf:type owl:Class ;
                           rdfs:subClassOf vocals-sd:StreamingService ;
                           rdfs:comment "An RDFStreamService represents a service that allows producing and/or consuming and/or processing RDF streams, and made available via an RDF streaming protocol."@en ;
                           rdfs:label "RDFStreamService"@en .


###  http://w3id.org/rsp/vocals-sd#RDFStreamingFeature
vocals-sd:RDFStreamingFeature rdf:type owl:Class ;
                              rdfs:comment "Represents a feature of a RDF Streaming service. Features may include operations over RDF streams, policies, time handling mechanisms, etc."@en ;
                              rdfs:label "RDFStreamingFeature"@en ;
                              rdfs:seeAlso vocals-sd:RDFStreamService .


###  http://w3id.org/rsp/vocals-sd#ReportingPolicy
vocals-sd:ReportingPolicy rdf:type owl:Class ;
                          rdfs:subClassOf vocals-sd:RDFStreamingFeature ;
                          rdfs:comment "The reporting policy establishes a strategy according to which data items are reported, typically within a window. E.g. report data items when teh window closes, periodically, when the window contents change, etc."@en ;
                          rdfs:label "ReportingPolicy"@en ;
                          rdfs:seeAlso vocals-sd:Window .


###  http://w3id.org/rsp/vocals-sd#S2ROperation
vocals-sd:S2ROperation rdf:type owl:Class ;
                       rdfs:subClassOf vocals-sd:Operation ;
                       rdfs:comment "An S2ROperation represents a stream-to-relation operation that an RDFStreamService can perform. It takes as input an RDF steam and putputs RDF data mapping, for instance windowing operators."@en ;
                       rdfs:isDefinedBy "Dell'Aglio, Daniele, et al. \"RSP-QL semantics: a unifying query model to explain heterogeneity of RDF stream processing systems.\" International Journal on Semantic Web and Information Systems (IJSWIS) 10.4 (2014): 17-44." ;
                       rdfs:label "S2ROperation"@en .


###  http://w3id.org/rsp/vocals-sd#S2SOperation
vocals-sd:S2SOperation rdf:type owl:Class ;
                       rdfs:subClassOf vocals-sd:Operation ;
                       rdfs:comment "An S2SOperation represents a stream-to-stream operation that an RDFStreamService can perform. It takes as input and output RDF streams (e.g. transformation operations over RDF streams)."@en ;
                       rdfs:label "S2SOperation"@en .


###  http://w3id.org/rsp/vocals-sd#SetOperation
vocals-sd:SetOperation rdf:type owl:Class ;
                       rdfs:subClassOf vocals-sd:S2SOperation ;
                       rdfs:comment "An instance of vsd:SetOperation represents an available set operator that can be performed by vsd:RSService. (e.g. union, intersection)" ;
                       rdfs:label "Set operation" .


###  http://w3id.org/rsp/vocals-sd#StreamingDataset
vocals-sd:StreamingDataset rdf:type owl:Class ;
                           owl:disjointWith <http://www.w3.org/ns/dcat#Dataset> ;
                           rdfs:comment "A Streaming Dataset provides the input data (from stream and time-varying graphs) for an RDF stream service. A Streaming Dataset is a set composed by an (optional) default graph, n (n ≥ 0) named graphs and m (m ≥ 0) named time-varying graphs."@en ;
                           rdfs:label "StreamingDataset"@en ;
                           rdfs:seeAlso vocals-sd:RDFStreamService ,
                                        vocals-sd:TimeVaryingGraph .


###  http://w3id.org/rsp/vocals-sd#StreamingService
vocals-sd:StreamingService rdf:type owl:Class ;
                           rdfs:comment "A StreamingService represents a service made available via a certain streaming protocol. The service may provide features such as stream processing, publishing, provisioning, etc."@en ;
                           rdfs:label "StreamingService"@en .


###  http://w3id.org/rsp/vocals-sd#TimeBasedWindow
vocals-sd:TimeBasedWindow rdf:type owl:Class ;
                          rdfs:subClassOf vocals-sd:Window ;
                          rdfs:comment "A TimeBasedWindow is a Window defined in terms of time. More formally, it is a window defined through two time instants o, c (respectively named opening and closing time instants) such that: W(S) = {d|(d, t) ∈ S ∧ t ∈ (o, c]}"@en ;
                          rdfs:label "TimeBasedWindow"@en ;
                          rdfs:seeAlso vocals-sd:Window .


###  http://w3id.org/rsp/vocals-sd#TimeControl
vocals-sd:TimeControl rdf:type owl:Class ;
                      rdfs:subClassOf vocals-sd:RDFStreamingFeature ;
                      rdfs:comment "TimeControl is a feature that establishes the type of timing control in the RDF stream Service, e.g. time managed internally, externally, etc."@en ;
                      rdfs:label "TimeControl"@en .


###  http://w3id.org/rsp/vocals-sd#TimeSemantics
vocals-sd:TimeSemantics rdf:type owl:Class ;
                        rdfs:subClassOf vocals-sd:RDFStreamingFeature ;
                        rdfs:comment "An instance of TimeSemantics represent the time domain used by streaming service while handeling the data elements, e.g. event time, porcessing time"@en ;
                        rdfs:isDefinedBy "The world beyond batch: Streaming 101 (https://www.oreilly.com/ideas/the-world-beyond-batch-streaming-101)" ;
                        rdfs:label "TimeSemantics"@en ;
                        rdfs:seeAlso vocals-sd:RDFStreamService .


###  http://w3id.org/rsp/vocals-sd#TimeVaryingGraph
vocals-sd:TimeVaryingGraph rdf:type owl:Class ;
                           rdfs:comment "A TimeVaryingGraph represents and RDF graph that changes over time. Formally, A time-varying graph G is a function that relates time instants t ∈ T to RDF graphs: G : T → {g | g is an RDF graph}, where T is the time domain."@en ;
                           rdfs:label "TimeVaryingGraph"@en .


###  http://w3id.org/rsp/vocals-sd#Window
vocals-sd:Window rdf:type owl:Class ;
                 rdfs:subClassOf <http://www.w3.org/ns/dcat#Dataset> ;
                 rdfs:comment "A Window represents a finite protion of a stream, consisting of a set of RDF statements. Formally, a window W(S) is a set of RDF statements extracted from a stream S."@en ;
                 rdfs:label "Window"@en ;
                 rdfs:seeAlso <http://w3id.org/rsp/vocals#RDFStream> .


###  http://www.w3.org/2006/time#Instant
time:Instant rdf:type owl:Class .


###  http://www.w3.org/ns/dcat#Dataset
<http://www.w3.org/ns/dcat#Dataset> rdf:type owl:Class .


###  http://www.w3.org/ns/formats/Format
frmt:Format rdf:type owl:Class .


#################################################################
#    Individuals
#################################################################

###  http://w3id.org/rsp/vocals-sd#RSPQL
vocals-sd:RSPQL rdf:type owl:NamedIndividual ,
                         vocals-sd:S2SOperation .


###  http://w3id.org/rsp/vocals-sd#background_data_support
vocals-sd:background_data_support rdf:type owl:NamedIndividual ,
                                           vocals-sd:RDFStreamingFeature ;
                                  rdfs:comment """An SFP system can either support or ignore
background data; assume that such data is fixed and available ex-ante; or allow
(infrequent) changes to this data.""" .


###  http://w3id.org/rsp/vocals-sd#completeness
vocals-sd:completeness rdf:type owl:NamedIndividual ,
                                vocals-sd:RDFStreamingFeature ;
                       rdfs:comment "Completeness measures whether the system guarantees a certain proportion of all correct answers" .


###  http://w3id.org/rsp/vocals-sd#count
vocals-sd:count rdf:type owl:NamedIndividual ,
                         vocals-sd:R2ROperation .


###  http://w3id.org/rsp/vocals-sd#declarative_languages
vocals-sd:declarative_languages rdf:type owl:NamedIndividual ,
                                         vocals-sd:QueryModel ;
                                rdfs:comment "Conversely, systems like C-SPARQL [10] extend declarative languages like SQL, augmenting them with operators like windows to limit the scope of processing." .


###  http://w3id.org/rsp/vocals-sd#difference
vocals-sd:difference rdf:type owl:NamedIndividual ,
                              vocals-sd:SetOperation .


###  http://w3id.org/rsp/vocals-sd#event_time
vocals-sd:event_time rdf:type owl:NamedIndividual ,
                              vocals-sd:TimeSemantics .


###  http://w3id.org/rsp/vocals-sd#external_time_control
vocals-sd:external_time_control rdf:type owl:NamedIndividual ,
                                         vocals-sd:TimeControl .


###  http://w3id.org/rsp/vocals-sd#filtering
vocals-sd:filtering rdf:type owl:NamedIndividual ,
                             vocals-sd:S2SOperation .


###  http://w3id.org/rsp/vocals-sd#ingestion_time
vocals-sd:ingestion_time rdf:type owl:NamedIndividual ,
                                  vocals-sd:TimeSemantics .


###  http://w3id.org/rsp/vocals-sd#internal_time_control
vocals-sd:internal_time_control rdf:type owl:NamedIndividual ,
                                         vocals-sd:TimeControl .


###  http://w3id.org/rsp/vocals-sd#intersection
vocals-sd:intersection rdf:type owl:NamedIndividual ,
                                vocals-sd:SetOperation .


###  http://w3id.org/rsp/vocals-sd#interval_based_semantics
vocals-sd:interval_based_semantics rdf:type owl:NamedIndividual ,
                                            vocals-sd:TimeSemantics ;
                                   rdfs:comment "The interval-based semantics defines an interval of validity for the associated information." .


###  http://w3id.org/rsp/vocals-sd#non_empty_content
vocals-sd:non_empty_content rdf:type owl:NamedIndividual ,
                                     vocals-sd:ReportingPolicy .


###  http://w3id.org/rsp/vocals-sd#on_content_change
vocals-sd:on_content_change rdf:type owl:NamedIndividual ,
                                     vocals-sd:ReportingPolicy .


###  http://w3id.org/rsp/vocals-sd#on_window_close
vocals-sd:on_window_close rdf:type owl:NamedIndividual ,
                                   vocals-sd:ReportingPolicy .


###  http://w3id.org/rsp/vocals-sd#pattern_matching
vocals-sd:pattern_matching rdf:type owl:NamedIndividual ,
                                    vocals-sd:QueryModel ;
                           rdfs:comment "Systems like EP-SPARQL define pattern matching queries through a set of primitive operators (e.g. sequences)." .


###  http://w3id.org/rsp/vocals-sd#periodic
vocals-sd:periodic rdf:type owl:NamedIndividual ,
                            vocals-sd:ReportingPolicy .


###  http://w3id.org/rsp/vocals-sd#periodic_evaluation
vocals-sd:periodic_evaluation rdf:type owl:NamedIndividual ,
                                       vocals-sd:QueryModel ;
                              rdfs:comment "The query is executed at a specified interval of time" .


###  http://w3id.org/rsp/vocals-sd#point_based_semantics
vocals-sd:point_based_semantics rdf:type owl:NamedIndividual ,
                                         vocals-sd:TimeSemantics ;
                                rdfs:comment """The point based semantics associates each information
item in the data-flow a single point in time""" .


###  http://w3id.org/rsp/vocals-sd#processing_time
vocals-sd:processing_time rdf:type owl:NamedIndividual ,
                                   vocals-sd:TimeSemantics .


###  http://w3id.org/rsp/vocals-sd#reactive_evaluation
vocals-sd:reactive_evaluation rdf:type owl:NamedIndividual ,
                                       vocals-sd:QueryModel ;
                              rdfs:comment "The query is triggered when new data arrives." .


###  http://w3id.org/rsp/vocals-sd#reasoning
vocals-sd:reasoning rdf:type owl:NamedIndividual ,
                             vocals-sd:RDFStreamingFeature ;
                    rdfs:comment """The usage of semantically annotated data allows
the SFP system to infer implicit information. This process is broadly referred as inference or reasoning. The ability of performing inference is feature unique to SFP system and not available in IFP systems. We make, however, no assumption about the expressive power of the inference mechanism.""" .


###  http://w3id.org/rsp/vocals-sd#replaying
vocals-sd:replaying rdf:type owl:NamedIndividual ,
                             vocals-sd:R2SOperation .


###  http://w3id.org/rsp/vocals-sd#soundness
vocals-sd:soundness rdf:type owl:NamedIndividual ,
                             vocals-sd:RDFStreamingFeature ;
                    rdfs:comment """soundness measures the number of incorrect results due, for ex-
ample, to approximation.""" .


###  http://w3id.org/rsp/vocals-sd#sum
vocals-sd:sum rdf:type owl:NamedIndividual ,
                       vocals-sd:R2ROperation .


###  http://w3id.org/rsp/vocals-sd#transform
vocals-sd:transform rdf:type owl:NamedIndividual ,
                             vocals-sd:S2SOperation .


###  http://w3id.org/rsp/vocals-sd#union
vocals-sd:union rdf:type owl:NamedIndividual ,
                         vocals-sd:SetOperation .


###  http://w3id.org/rsp/vocals-sd#windowing
vocals-sd:windowing rdf:type owl:NamedIndividual ,
                             vocals-sd:S2ROperation .


###  Generated by the OWL API (version 4.2.8.20170104-2310) https://github.com/owlcs/owlapi
