@prefix : <http://w3id.org/rsp/vocals-prov#> .
@prefix dc: <http://purl.org/dc/elements/1.1/> .
@prefix owl: <http://www.w3.org/2002/07/owl#> .
@prefix rdf: <http://www.w3.org/1999/02/22-rdf-syntax-ns#> .
@prefix vsd: <http://w3id.org/rsp/vocals-sd#> .
@prefix xml: <http://www.w3.org/XML/1998/namespace> .
@prefix xsd: <http://www.w3.org/2001/XMLSchema#> .
@prefix prov: <http://www.w3.org/ns/prov#> .
@prefix rdfs: <http://www.w3.org/2000/01/rdf-schema#> .
@prefix time: <http://www.w3.org/2006/time#> .
@prefix vann: <http://purl.org/vocab/vann/> .
@prefix vocals: <http://w3id.org/rsp/vocals#> .
@prefix dcterms: <http://purl.org/dc/terms/> .
@base <http://w3id.org/rsp/vocals-prov#> .

<http://w3id.org/rsp/vocals-prov#> rdf:type owl:Ontology ;
                                    owl:versionIRI <http://w3id.org/rsp/vocals-prov> ;
                                    dc:publisher <http://aislab.hevs.ch/> ;
                                    dc:creator <https://w3id.org/people/rictomm> ;
                                    vann:preferredNamespaceUri "http://w3id.org/rsp/vocals-prov#" ;
                                    dcterms:modified "2017-12-30"^^xsd:date ;
                                    dc:creator <http://w3id.org/people/jpcik/me> ;
                                    dcterms:rights "Copyright © 2017 Politecnico di Milano & HES-SO Valais-Wallis"^^xsd:string ;
                                    dcterms:description "Cette ontologie a été conçue pour representer la provenance de données et meta-données de streams RDF, ainsi que leurs points d'accès."@fr ;
                                    dcterms:title "VoCaLS-Prov: Vocabulario y catálogo para Streams enlazados, módulo de Provenance"@es ,
                                                  "VoCaLS-Prov: A Vocabulary and Catalog for Linked Streams, Provenance Module"@en ;
                                    dcterms:description "Esta ontología has sido diseñada para representar provenance de Streams de datos en RDF, así como los endpoints a través de los cuales se puede acceder a los datos de estos streams;  y los meta datos correspondientes."@es ;
                                    rdfs:comment "Cette ontologie a été conçue pour representer la provenance de données et meta-données de streams RDF, ainsi que leurs points d'accès."@fr ,
                                                 "Esta ontología has sido diseñada para representar provenance de Streams de datos en RDF, así como los endpoints a través de los cuales se puede acceder a los datos de estos streams;  y los meta datos correspondientes."@es ;
                                    dcterms:license <https://creativecommons.org/licenses/by/4.0/> ;
                                    dcterms:publisher <http://w3id.org/hes-so/aislab> ;
                                    dcterms:created "2017-12-23T13:00:00"^^xsd:dateTime ;
                                    dcterms:issued "2017-12-29"^^xsd:date ;
                                    rdfs:comment "This ontology aims to model provenance of RDF streams, their metadata, and access endpoints for publishing and consuming these streams"@en ;
                                    dc:creator <http://w3id.org/rsp/vocals#YehiaAboSedira> ;
                                    dcterms:title "VoCaLS-Prov: ontologie de representation de provenance pour données et metadonnées de streams RDF"@fr ;
                                    vann:preferredNamespacePrefix "vocals-prov" ;
                                    owl:versionInfo "0.1.1"^^xsd:string ;
                                    dcterms:description "This ontology aims to model provenance of RDF streams, their metadata, and access endpoints for publishing and consuming these streams"@en .

#################################################################
#    Object Properties
#################################################################

###  http://w3id.org/rsp/vocals-prov#containedIn
:containedIn rdf:type owl:ObjectProperty ;
             owl:inverseOf :contains ;
             rdfs:domain :Operator ;
             rdfs:range :Task ;
             rdfs:comment "Relates an Operator to the containing Task."@en ;
             rdfs:label "containedIn"@en .


###  http://w3id.org/rsp/vocals-prov#contains
:contains rdf:type owl:ObjectProperty ;
          rdfs:domain :Task ;
          rdfs:range :Operator ;
          rdfs:comment "Relates a Task to Operator used to finish the task."@en ;
          rdfs:label "contains"@en .


###  http://w3id.org/rsp/vocals-prov#endedAt
:endedAt rdf:type owl:ObjectProperty ;
         rdfs:domain :Window ;
         rdfs:range time:Instant .


###  http://w3id.org/rsp/vocals-prov#followedBy
:followedBy rdf:type owl:ObjectProperty ;
            owl:inverseOf :precededBy ;
            rdfs:domain :Operator ;
            rdfs:range :Operator ;
            rdfs:comment "Points to the following :operator to be applied after the current one in a :Task." .


###  http://w3id.org/rsp/vocals-prov#hasOutput
:hasOutput rdf:type owl:ObjectProperty ;
           rdfs:domain :Task ;
           rdfs:range prov:Entity ;
           rdfs:comment "Points to the output of a :operator to be applied before the current one in a :Task." .


###  http://w3id.org/rsp/vocals-prov#performs
:performs rdf:type owl:ObjectProperty ;
          rdfs:range vsd:Operation ;
          rdfs:isDefinedBy "Relate vsd:Operation to :Operator ." .


###  http://w3id.org/rsp/vocals-prov#precededBy
:precededBy rdf:type owl:ObjectProperty ;
            rdfs:domain :Operator ;
            rdfs:range :Operator ;
            rdfs:comment "Points to the preceding :operator to be applied before the current one in a :Task." .


###  http://w3id.org/rsp/vocals-prov#startedAt
:startedAt rdf:type owl:ObjectProperty ;
           rdfs:domain :Window ;
           rdfs:range time:Instant .


###  http://w3id.org/rsp/vocals-prov#startingTime
:startingTime rdf:type owl:ObjectProperty ;
              rdfs:domain :WindowOperator ;
              rdfs:range time:Instant .


#################################################################
#    Data properties
#################################################################

###  http://w3id.org/rsp/vocals-prov#query
:query rdf:type owl:DatatypeProperty ;
       rdfs:subPropertyOf owl:topDataProperty ;
       rdfs:domain :RSPQLOperator .


###  http://w3id.org/rsp/vocals-prov#range
:range rdf:type owl:DatatypeProperty ;
       rdfs:subPropertyOf owl:topDataProperty ;
       rdfs:domain :WindowOperator .


###  http://w3id.org/rsp/vocals-prov#step
:step rdf:type owl:DatatypeProperty ;
      rdfs:subPropertyOf owl:topDataProperty ;
      rdfs:domain :WindowOperator .


#################################################################
#    Classes
#################################################################

###  http://w3id.org/rsp/vocals-prov#FilterOperator
:FilterOperator rdf:type owl:Class ;
                rdfs:subClassOf :S2SOperator ;
                rdfs:comment "A :FilterOperator represents an operator that exclude data that doesn't match some specified criteria." .


###  http://w3id.org/rsp/vocals-prov#Operator
:Operator rdf:type owl:Class ;
          rdfs:subClassOf prov:Activity ;
          rdfs:comment "Operator that use a resource - stream, relation - to generate another resource." .


###  http://w3id.org/rsp/vocals-prov#PhysicalWindow
:PhysicalWindow rdf:type owl:Class ;
                rdfs:subClassOf :Window ;
                rdfs:comment "Window defined by an interval size (in units of RDF elements)" .


###  http://w3id.org/rsp/vocals-prov#R2ROperator
:R2ROperator rdf:type owl:Class ;
             rdfs:subClassOf :Operator ;
             rdfs:comment "Operators that produce relations from other relations." ;
             rdfs:isDefinedBy "Arvind Arasu, Shivnath Babu, and Jennifer Widom. 2006. The CQL continuous query language: semantic foundations and query execution. The VLDB Journal 15, 2 (June 2006), 121-142. DOI=http://dx.doi.org/10.1007/s00778-004-0147-z" .


###  http://w3id.org/rsp/vocals-prov#R2SOperator
:R2SOperator rdf:type owl:Class ;
             rdfs:subClassOf :Operator ;
             rdfs:comment "Operators that produce a stream from a relation." ;
             rdfs:isDefinedBy "Arvind Arasu, Shivnath Babu, and Jennifer Widom. 2006. The CQL continuous query language: semantic foundations and query execution. The VLDB Journal 15, 2 (June 2006), 121-142. DOI=http://dx.doi.org/10.1007/s00778-004-0147-z" .


###  http://w3id.org/rsp/vocals-prov#RSPQLOperator
:RSPQLOperator rdf:type owl:Class ;
               rdfs:subClassOf :S2SOperator ;
               owl:disjointWith :SetOperator ;
               rdfs:comment "RDF Stream Processing (RSP) Operators that produce a stream by appling a C-Sparql query to another stream." ;
               rdfs:label "RSPQL operator" .


###  http://w3id.org/rsp/vocals-prov#Replay
:Replay rdf:type owl:Class ;
        rdfs:subClassOf :R2SOperator ;
        rdfs:comment "Replay operator produce a stream from a static RDF dataset" ;
        rdfs:isDefinedBy "https://link.springer.com/chapter/10.1007%2F978-3-319-46547-0_15" .


###  http://w3id.org/rsp/vocals-prov#S2ROperator
:S2ROperator rdf:type owl:Class ;
             rdfs:subClassOf :Operator ;
             rdfs:comment "Operators that produce a relation from a stream." ;
             rdfs:isDefinedBy "Arvind Arasu, Shivnath Babu, and Jennifer Widom. 2006. The CQL continuous query language: semantic foundations and query execution. The VLDB Journal 15, 2 (June 2006), 121-142. DOI=http://dx.doi.org/10.1007/s00778-004-0147-z" .


###  http://w3id.org/rsp/vocals-prov#S2SOperator
:S2SOperator rdf:type owl:Class ;
             rdfs:subClassOf :Operator ;
             rdfs:comment "Operators that produce a stream form another stream." .


###  http://w3id.org/rsp/vocals-prov#SetOperator
:SetOperator rdf:type owl:Class ;
             rdfs:subClassOf :S2SOperator ;
             rdfs:comment "Operator that produce a stream by applying set algebra operator on other streams." .


###  http://w3id.org/rsp/vocals-prov#StreamingAgent
:StreamingAgent rdf:type owl:Class ;
                rdfs:subClassOf prov:SoftwareAgent ;
                rdfs:comment "An instance of a :StreamingAgent represent an actor that applies an :Operator that consums and/or produce a stream." ;
                rdfs:label "StreamingAgent"@en .


###  http://w3id.org/rsp/vocals-prov#Task
:Task rdf:type owl:Class ;
      rdfs:comment "A task contains one or more activity to be applied on a prov:Entity." .


###  http://w3id.org/rsp/vocals-prov#TimeBasedWindow
:TimeBasedWindow rdf:type owl:Class ;
                 rdfs:subClassOf :Window ;
                 rdfs:comment "A time-based window is a window defined through two time instants o, c (respectively named opening and closing time instants) such that: W(S) = {d|(d, t) ∈ S ∧ t ∈ (o, c]}" .


###  http://w3id.org/rsp/vocals-prov#TransformOperator
:TransformOperator rdf:type owl:Class ;
                   rdfs:subClassOf :S2SOperator ;
                   rdfs:comment "An instance of :TransformOperator represent an operator that convert a stream from one form to another. (e.g. Convert a raw stream to and RDF stream)" .


###  http://w3id.org/rsp/vocals-prov#Window
:Window rdf:type owl:Class ;
        rdfs:subClassOf <http://www.w3.org/ns/dcat#Dataset> ;
        rdfs:comment "A window W(S) is a set of RDF statements extracted from a stream S." .


###  http://w3id.org/rsp/vocals-prov#WindowOperator
:WindowOperator rdf:type owl:Class ;
                rdfs:subClassOf :S2ROperator ;
                rdfs:comment "An instance of window operator represent an operator that use a stream and generate multiple windows according to a certain criteria" .


###  http://w3id.org/rsp/vocals-sd#Operation
vsd:Operation rdf:type owl:Class .


###  http://www.w3.org/2006/time#Instant
time:Instant rdf:type owl:Class .


###  http://www.w3.org/ns/dcat#Dataset
<http://www.w3.org/ns/dcat#Dataset> rdf:type owl:Class .


###  http://www.w3.org/ns/prov#Activity
prov:Activity rdf:type owl:Class .


###  http://www.w3.org/ns/prov#Entity
prov:Entity rdf:type owl:Class .


###  http://www.w3.org/ns/prov#SoftwareAgent
prov:SoftwareAgent rdf:type owl:Class .


#################################################################
#    Individuals
#################################################################

###  http://w3id.org/rsp/vocals-prov#TripleWave
:TripleWave rdf:type owl:NamedIndividual ,
                     :StreamingAgent .


###  http://w3id.org/rsp/vocals-prov#difference_operator
:difference_operator rdf:type owl:NamedIndividual ,
                              :SetOperator .


###  http://w3id.org/rsp/vocals-prov#intersect_operator
:intersect_operator rdf:type owl:NamedIndividual ,
                             :SetOperator .


###  http://w3id.org/rsp/vocals-prov#union_operator
:union_operator rdf:type owl:NamedIndividual ,
                         :SetOperator .


###  Generated by the OWL API (version 4.2.8.20170104-2310) https://github.com/owlcs/owlapi
