@prefix : <https://w3id.org/rsp/vocals-sd#> .
@prefix sd: <http://www.w3.org/ns/sparql-service-description#> .
@prefix owl: <http://www.w3.org/2002/07/owl#> .
@prefix rdf: <http://www.w3.org/1999/02/22-rdf-syntax-ns#> .
@prefix xml: <http://www.w3.org/XML/1998/namespace> .
@prefix xsd: <http://www.w3.org/2001/XMLSchema#> .
@prefix frmt: <http://www.w3.org/ns/formats/> .
@prefix rdfs: <http://www.w3.org/2000/01/rdf-schema#> .
@prefix time: <http://www.w3.org/2006/time#> .
@prefix vocals: <https://w3id.org/rsp/vocals#> .
@prefix vocals-sd: <https://w3id.org/rsp/vocals-sd#> .
@base <https://w3id.org/rsp/vocals-sd> .

<https://w3id.org/rsp/vocals-sd> rdf:type owl:Ontology ;
                                  owl:versionIRI <https://w3id.org/rsp/vocals-sd> ;
                                  <http://purl.org/vocab/vann/preferredNamespaceUri> "https://w3id.org/rsp/vocals-sd#" ;
                                  <http://purl.org/dc/elements/1.1/creator> vocals:RiccardoTommasini ,
                                                                            vocals:EmanueleDellaValle ;
                                  <http://purl.org/vocab/vann/preferredNamespacePrefix> "vois-sd" ;
                                  <http://purl.org/dc/terms/created> "2017-05-23T13:00:00"^^xsd:dateTime ;
                                  <http://purl.org/dc/elements/1.1/creator> vocals:YehiaAboSedira .

#################################################################
#    Annotation properties
#################################################################

###  http://www.w3.org/ns/sparql-service-description#name
sd:name rdf:type owl:AnnotationProperty ;
        rdfs:comment "Relates a named graph to the name by which it may be referenced in a FROM/FROM NAMED clause. The object of the sd:name property is an IRI." ;
        rdfs:label "name" ;
        rdfs:domain sd:NamedGraph .


#################################################################
#    Object Properties
#################################################################

###  http://www.w3.org/ns/sparql-service-description#availableGraphs
sd:availableGraphs rdf:type owl:ObjectProperty ;
                   rdfs:domain sd:Service ;
                   rdfs:range sd:GraphCollection ;
                   rdfs:comment "Relates an instance of sd:Service to a description of the graphs which are allowed in the construction of a dataset either via the SPARQL Protocol, with FROM/FROM NAMED clauses in a query, or with USING/USING NAMED in an update request, if the service limits the scope of dataset construction." ;
                   rdfs:label "available graph descriptions" .


###  http://www.w3.org/ns/sparql-service-description#defaultDataset
sd:defaultDataset rdf:type owl:ObjectProperty ,
                           owl:InverseFunctionalProperty ;
                  rdfs:domain sd:Service ;
                  rdfs:range sd:Dataset ;
                  rdfs:comment "Relates an instance of sd:Service to a description of the default dataset available when no explicit dataset is specified in the query, update request or via protocol parameters." ;
                  rdfs:label "default dataset description" .


###  http://www.w3.org/ns/sparql-service-description#defaultEntailmentRegime
sd:defaultEntailmentRegime rdf:type owl:ObjectProperty ;
                           rdfs:subPropertyOf sd:feature ;
                           rdfs:domain sd:Service ;
                           rdfs:range sd:EntailmentRegime ;
                           rdfs:comment "Relates an instance of sd:Service with a resource representing an entailment regime used for basic graph pattern matching. This property is intended for use when a single entailment regime by default applies to all graphs in the default dataset of the service. In situations where a different entailment regime applies to a specific graph in the dataset, the sd:entailmentRegime property should be used to indicate this fact in the description of that graph." ;
                           rdfs:label "default entailment regime" .


###  http://www.w3.org/ns/sparql-service-description#defaultGraph
sd:defaultGraph rdf:type owl:ObjectProperty ;
                rdfs:domain sd:Dataset ;
                rdfs:range sd:Graph ;
                rdfs:comment "Relates an instance of sd:Dataset to the description of its default graph." ;
                rdfs:label "default graph" .


###  http://www.w3.org/ns/sparql-service-description#defaultSupportedEntailmentProfile
sd:defaultSupportedEntailmentProfile rdf:type owl:ObjectProperty ;
                                     rdfs:subPropertyOf sd:feature ;
                                     rdfs:domain sd:Service ;
                                     rdfs:range sd:EntailmentProfile ;
                                     rdfs:comment "Relates an instance of sd:Service with a resource representing a supported profile of the default entailment regime (as declared by sd:defaultEntailmentRegime)." ;
                                     rdfs:label "default supported entailment profile" .


###  http://www.w3.org/ns/sparql-service-description#endpoint
sd:endpoint rdf:type owl:ObjectProperty ,
                     owl:InverseFunctionalProperty ;
            rdfs:domain sd:Service ;
            rdfs:comment "The SPARQL endpoint of an sd:Service that implements the SPARQL Protocol service. The object of the sd:endpoint property is an IRI." ;
            rdfs:label "endpoint" .


###  http://www.w3.org/ns/sparql-service-description#extensionAggregate
sd:extensionAggregate rdf:type owl:ObjectProperty ;
                      rdfs:subPropertyOf sd:feature ;
                      rdfs:domain sd:Service ;
                      rdfs:range sd:Aggregate ;
                      rdfs:comment "Relates an instance of sd:Service to an aggregate that may be used in a SPARQL aggregate query (for instance in a HAVING clause or SELECT expression) besides the standard list of supported aggregates COUNT, SUM, MIN, MAX, AVG, GROUP_CONCAT, and SAMPLE" ;
                      rdfs:label "extension aggregate" .


###  http://www.w3.org/ns/sparql-service-description#extensionFunction
sd:extensionFunction rdf:type owl:ObjectProperty ;
                     rdfs:subPropertyOf sd:feature ;
                     rdfs:domain sd:Service ;
                     rdfs:range sd:Function ;
                     rdfs:comment "Relates an instance of sd:Service to a function that may be used in a SPARQL SELECT expression or a FILTER, HAVING, GROUP BY, ORDER BY, or BIND clause." ;
                     rdfs:label "extension function" .


###  http://www.w3.org/ns/sparql-service-description#feature
sd:feature rdf:type owl:ObjectProperty ;
           rdfs:domain sd:Service ;
           rdfs:range sd:Feature ;
           rdfs:comment "Relates an instance of sd:Service with a resource representing a supported feature." ;
           rdfs:label "feature" .


###  http://www.w3.org/ns/sparql-service-description#graph
sd:graph rdf:type owl:ObjectProperty ;
         rdfs:domain sd:NamedGraph ;
         rdfs:range sd:Graph ;
         rdfs:comment "Relates a named graph to its graph description." ;
         rdfs:label "graph" .


###  http://www.w3.org/ns/sparql-service-description#inputFormat
sd:inputFormat rdf:type owl:ObjectProperty ;
               rdfs:domain sd:Service ;
               rdfs:range frmt:Format ;
               rdfs:comment "Relates an instance of sd:Service to a format that is supported for parsing RDF input; for example, via a SPARQL 1.1 Update LOAD statement, or when URIs are dereferenced in FROM/FROM NAMED/USING/USING NAMED clauses." ;
               rdfs:label "input format" .


###  http://www.w3.org/ns/sparql-service-description#languageExtension
sd:languageExtension rdf:type owl:ObjectProperty ;
                     rdfs:subPropertyOf sd:feature ;
                     rdfs:domain sd:Service ;
                     rdfs:range sd:Feature ;
                     rdfs:comment "Relates an instance of sd:Service to a resource representing an implemented extension to the SPARQL Query or Update language." ;
                     rdfs:label "language extension" .


###  http://www.w3.org/ns/sparql-service-description#namedGraph
sd:namedGraph rdf:type owl:ObjectProperty ;
              rdfs:domain sd:GraphCollection ;
              rdfs:range sd:NamedGraph ;
              rdfs:comment "Relates an instance of sd:GraphCollection (or its subclass sd:Dataset) to the description of one of its named graphs. The description of such a named graph MUST include the sd:name property and MAY include the sd:graph property." ;
              rdfs:label "named graph" .


###  http://www.w3.org/ns/sparql-service-description#propertyFeature
sd:propertyFeature rdf:type owl:ObjectProperty ;
                   rdfs:subPropertyOf sd:feature ;
                   rdfs:domain sd:Service ;
                   rdfs:range sd:Feature ;
                   rdfs:comment "Relates an instance of sd:Service to a resource representing an implemented feature that extends the SPARQL Query or Update language and that is accessed by using the named property." ;
                   rdfs:label "property feature" .


###  http://www.w3.org/ns/sparql-service-description#resultFormat
sd:resultFormat rdf:type owl:ObjectProperty ;
                rdfs:domain sd:Service ;
                rdfs:range frmt:Format ;
                rdfs:comment "Relates an instance of sd:Service to a format that is supported for serializing query results." ;
                rdfs:label "result format" .


###  http://www.w3.org/ns/sparql-service-description#supportedLanguage
sd:supportedLanguage rdf:type owl:ObjectProperty ;
                     rdfs:subPropertyOf sd:feature ;
                     rdfs:domain sd:Service ;
                     rdfs:range sd:Language ;
                     rdfs:comment "Relates an instance of sd:Service to a SPARQL language (e.g. Query and Update) that it implements." ;
                     rdfs:label "supported language" .


###  https://w3id.org/rsp/vocals-sd#availableGraphs
vocals-sd:availableGraphs rdf:type owl:ObjectProperty ;
                          rdfs:subPropertyOf owl:topObjectProperty ;
                          rdfs:domain vocals-sd:RSService ;
                          rdfs:range sd:Graph ,
                                     vocals-sd:TimeVaryingGraph .


###  https://w3id.org/rsp/vocals-sd#availableStreams
vocals-sd:availableStreams rdf:type owl:ObjectProperty .


###  https://w3id.org/rsp/vocals-sd#defaultGraph
vocals-sd:defaultGraph rdf:type owl:ObjectProperty ;
                       rdfs:domain vocals:RDFStream ;
                       rdfs:range sd:Graph ;
                       rdfs:comment "Relates an instance of vocals:RDFStream to the description of its default graph." .


###  https://w3id.org/rsp/vocals-sd#describedBy
vocals-sd:describedBy rdf:type owl:ObjectProperty ;
                      rdfs:subPropertyOf owl:topObjectProperty ;
                      rdfs:domain vocals-sd:CatalogService ;
                      rdfs:range vocals:RDFStream ;
                      rdfs:comment "Points to an instance of vois-sd:CatalogingService that describes a certain vocals:RDFStream." .


###  https://w3id.org/rsp/vocals-sd#endedAt
vocals-sd:endedAt rdf:type owl:ObjectProperty ;
                  rdfs:subPropertyOf owl:topObjectProperty ;
                  rdfs:domain vocals-sd:Window ;
                  rdfs:range time:Instant .


###  https://w3id.org/rsp/vocals-sd#graph
vocals-sd:graph rdf:type owl:ObjectProperty ;
                rdfs:subPropertyOf owl:topObjectProperty ;
                rdfs:domain sd:NamedGraph ;
                rdfs:range sd:Graph ;
                rdfs:comment "Relates a named graph to its graph description." .


###  https://w3id.org/rsp/vocals-sd#hasReportingPolicy
vocals-sd:hasReportingPolicy rdf:type owl:ObjectProperty ;
                             rdfs:subPropertyOf owl:topObjectProperty ;
                             rdfs:domain vocals-sd:RSService ;
                             rdfs:range vocals-sd:ReportingPolicy .


###  https://w3id.org/rsp/vocals-sd#namedGraph
vocals-sd:namedGraph rdf:type owl:ObjectProperty ;
                     rdfs:subPropertyOf owl:topObjectProperty ;
                     rdfs:domain vocals-sd:SDS ;
                     rdfs:range sd:NamedGraph ;
                     rdfs:comment "Relates an instance of vocals:Window to the description of one of its named graphs. The description of such a named graph MUST include the sd:name property." ;
                     rdfs:label "named graph" .


###  https://w3id.org/rsp/vocals-sd#namedTimeVaryingGraph
vocals-sd:namedTimeVaryingGraph rdf:type owl:ObjectProperty ;
                                rdfs:domain vocals-sd:SDS ;
                                rdfs:range vocals-sd:TimeVaryingGraph .


###  https://w3id.org/rsp/vocals-sd#publishedBy
vocals-sd:publishedBy rdf:type owl:ObjectProperty ;
                      rdfs:subPropertyOf owl:topObjectProperty ;
                      rdfs:domain vocals:RDFStream ;
                      rdfs:range vocals-sd:PublishingService ;
                      rdfs:comment "Points to an instance of vois-sd:PublishingService that publishs a certain vocals:RDFStream." .


###  https://w3id.org/rsp/vocals-sd#registeredBy
vocals-sd:registeredBy rdf:type owl:ObjectProperty ;
                       rdfs:subPropertyOf owl:topObjectProperty ;
                       rdfs:domain vocals:RDFStream ;
                       rdfs:range vocals-sd:ProcessingService ;
                       rdfs:comment "Points to an instance of vois-sd:ProcessingService that registers/ processes a certain vocals:RDFStream." .


###  https://w3id.org/rsp/vocals-sd#resultFormat
vocals-sd:resultFormat rdf:type owl:ObjectProperty ;
                       rdfs:domain vocals-sd:RSService ;
                       rdfs:range frmt:Format ;
                       rdfs:comment "Relates an instance of sd:Service to a format that is supported for serializing query results." ;
                       rdfs:label "result format" .


###  https://w3id.org/rsp/vocals-sd#rspEndpoint
vocals-sd:rspEndpoint rdf:type owl:ObjectProperty ;
                      rdfs:subPropertyOf owl:topObjectProperty ;
                      rdfs:domain vocals-sd:RSService ;
                      rdfs:comment "The RSP-QL endpoint of an vocals:RSPService that implements the RSP-QL Protocol service. The object of the vocals:rspEndpoint property is an IRI." ;
                      rdfs:label "RSP endpoint" .


###  https://w3id.org/rsp/vocals-sd#startedAt
vocals-sd:startedAt rdf:type owl:ObjectProperty ;
                    rdfs:subPropertyOf owl:topObjectProperty ;
                    rdfs:domain vocals-sd:Window ;
                    rdfs:range time:Instant .


###  https://w3id.org/rsp/vocals-sd#startingTime
vocals-sd:startingTime rdf:type owl:ObjectProperty ;
                       rdfs:subPropertyOf owl:topObjectProperty ;
                       rdfs:range time:Instant .


#################################################################
#    Data properties
#################################################################

###  https://w3id.org/rsp/vocals-sd#range
vocals-sd:range rdf:type owl:DatatypeProperty ;
                rdfs:range xsd:positiveInteger .


###  https://w3id.org/rsp/vocals-sd#step
vocals-sd:step rdf:type owl:DatatypeProperty ;
               rdfs:range xsd:positiveInteger .


#################################################################
#    Classes
#################################################################

###  http://www.w3.org/2006/time#Instant
time:Instant rdf:type owl:Class .


###  http://www.w3.org/ns/dcat#Dataset
<http://www.w3.org/ns/dcat#Dataset> rdf:type owl:Class .


###  http://www.w3.org/ns/formats/Format
frmt:Format rdf:type owl:Class .


###  http://www.w3.org/ns/sparql-service-description#Aggregate
sd:Aggregate rdf:type owl:Class ;
             rdfs:subClassOf sd:Feature ;
             rdfs:comment "An instance of sd:Aggregate represents an aggregate that may be used in a SPARQL aggregate query (for instance in a HAVING clause or SELECT expression) besides the standard list of supported aggregates COUNT, SUM, MIN, MAX, AVG, GROUP_CONCAT, and SAMPLE." ;
             rdfs:label "Aggregate" .


###  http://www.w3.org/ns/sparql-service-description#Dataset
sd:Dataset rdf:type owl:Class ;
           rdfs:subClassOf sd:GraphCollection ;
           rdfs:comment "An instance of sd:Dataset represents a RDF Dataset comprised of a default graph and zero or more named graphs." ;
           rdfs:label "Dataset" .


###  http://www.w3.org/ns/sparql-service-description#EntailmentProfile
sd:EntailmentProfile rdf:type owl:Class ;
                     rdfs:subClassOf sd:Feature ;
                     rdfs:comment "An instance of sd:EntailmentProfile represents a profile of an entailment regime. An entailment profile MAY impose restrictions on what constitutes valid RDF with respect to entailment." ;
                     rdfs:label "Entailment Profile" .


###  http://www.w3.org/ns/sparql-service-description#EntailmentRegime
sd:EntailmentRegime rdf:type owl:Class ;
                    rdfs:subClassOf sd:Feature ;
                    rdfs:comment "An instance of sd:EntailmentRegime represents an entailment regime used in basic graph pattern matching (as described by SPARQL 1.1 Query Language)." ;
                    rdfs:label "Entailment Regime" .


###  http://www.w3.org/ns/sparql-service-description#Feature
sd:Feature rdf:type owl:Class ;
           rdfs:comment "An instance of sd:Feature represents a feature of a SPARQL service. Specific types of features include functions, aggregates, languages, and entailment regimes and profiles. This document defines five instances of sd:Feature: sd:DereferencesURIs, sd:UnionDefaultGraph, sd:RequiresDataset, sd:EmptyGraphs, and sd:BasicFederatedQuery." ;
           rdfs:label "Feature" .


###  http://www.w3.org/ns/sparql-service-description#Function
sd:Function rdf:type owl:Class ;
            rdfs:subClassOf sd:Feature ;
            rdfs:comment "An instance of sd:Function represents a function that may be used in a SPARQL SELECT expression or a FILTER, HAVING, GROUP BY, ORDER BY, or BIND clause." ;
            rdfs:label "Function" .


###  http://www.w3.org/ns/sparql-service-description#Graph
sd:Graph rdf:type owl:Class ;
         rdfs:comment "An instance of sd:Graph represents the description of an RDF graph." ;
         rdfs:label "Graph" .


###  http://www.w3.org/ns/sparql-service-description#GraphCollection
sd:GraphCollection rdf:type owl:Class ;
                   rdfs:comment "An instance of sd:GraphCollection represents a collection of zero or more named graph descriptions. Each named graph description belonging to an sd:GraphCollection MUST be linked with the sd:namedGraph predicate." ;
                   rdfs:label "Graph Collection" .


###  http://www.w3.org/ns/sparql-service-description#Language
sd:Language rdf:type owl:Class ;
            rdfs:subClassOf sd:Feature ;
            rdfs:comment "An instance of sd:Language represents one of the SPARQL languages, including specific configurations providing particular features or extensions. This document defines three instances of sd:Language: sd:SPARQL10Query, sd:SPARQL11Query, and sd:SPARQL11Update." ;
            rdfs:label "Language" .


###  http://www.w3.org/ns/sparql-service-description#NamedGraph
sd:NamedGraph rdf:type owl:Class ;
              rdfs:comment "An instance of sd:NamedGraph represents a named graph having a name (via sd:name) and an optional graph description (via sd:graph)." ;
              rdfs:label "Named Graph" .


###  http://www.w3.org/ns/sparql-service-description#Service
sd:Service rdf:type owl:Class ;
           rdfs:comment "An instance of sd:Service represents a SPARQL service made available via the SPARQL Protocol." ;
           rdfs:label "Service" .


###  https://w3id.org/rsp/vocals#RDFStream
vocals:RDFStream rdf:type owl:Class .


###  https://w3id.org/rsp/vocals-sd#CatalogService
vocals-sd:CatalogService rdf:type owl:Class ;
                         rdfs:subClassOf vocals-sd:RSService ;
                         rdfs:comment "An vois-sd:CatalogService is a service storing stream descriptions." ;
                         rdfs:seeAlso "vocals:StreamDescriptor" .


###  https://w3id.org/rsp/vocals-sd#Operation
vocals-sd:Operation rdf:type owl:Class ;
                    rdfs:subClassOf vocals-sd:RSPFeature .


###  https://w3id.org/rsp/vocals-sd#PhysicalWindow
vocals-sd:PhysicalWindow rdf:type owl:Class ;
                         rdfs:subClassOf vocals-sd:Window ;
                         rdfs:comment "Window defined by an interval size (in units of RDF elements)" .


###  https://w3id.org/rsp/vocals-sd#ProcessingService
vocals-sd:ProcessingService rdf:type owl:Class ;
                            rdfs:subClassOf vocals-sd:RSService ;
                            rdfs:comment "An vois-sd:ProcessingService represents an RDF stream processing service. Processing means any kind of transformation on streaming data, i.e., Querying, Reasoning, Filtering...etc" .


###  https://w3id.org/rsp/vocals-sd#PublishingService
vocals-sd:PublishingService rdf:type owl:Class ;
                            rdfs:subClassOf vocals-sd:RSService ;
                            rdfs:comment "An vois-sd:PublishingService represents a stream publishing service. Publishing has to be interpreted as in Linked Data domain, where is possible." .


###  https://w3id.org/rsp/vocals-sd#R2ROperation
vocals-sd:R2ROperation rdf:type owl:Class ;
                       rdfs:subClassOf vocals-sd:Operation .


###  https://w3id.org/rsp/vocals-sd#R2SOperation
vocals-sd:R2SOperation rdf:type owl:Class ;
                       rdfs:subClassOf vocals-sd:Operation .


###  https://w3id.org/rsp/vocals-sd#RSPFeature
vocals-sd:RSPFeature rdf:type owl:Class .


###  https://w3id.org/rsp/vocals-sd#RSService
vocals-sd:RSService rdf:type owl:Class ;
                    rdfs:subClassOf vocals-sd:StreamingService ;
                    rdfs:comment "An instance of vois-sd:Service represents a RDF streaming service made available via RSP-QL protocol." .


###  https://w3id.org/rsp/vocals-sd#ReportingPolicy
vocals-sd:ReportingPolicy rdf:type owl:Class ;
                          rdfs:subClassOf vocals-sd:RSPFeature ;
                          rdfs:label "Reporting Policy" .


###  https://w3id.org/rsp/vocals-sd#S2ROperation
vocals-sd:S2ROperation rdf:type owl:Class ;
                       rdfs:subClassOf vocals-sd:Operation .


###  https://w3id.org/rsp/vocals-sd#S2SOperation
vocals-sd:S2SOperation rdf:type owl:Class ;
                       rdfs:subClassOf vocals-sd:Operation .


###  https://w3id.org/rsp/vocals-sd#SDS
vocals-sd:SDS rdf:type owl:Class ;
              rdfs:comment "A streaming dataset is a set composed by an (optional) default graph, n (n ≥ 0) named graphs and m (m ≥ 0) named time-varying graphs" ;
              rdfs:label "SDS" .


###  https://w3id.org/rsp/vocals-sd#SetOperation
vocals-sd:SetOperation rdf:type owl:Class ;
                       rdfs:subClassOf vocals-sd:S2SOperation .


###  https://w3id.org/rsp/vocals-sd#StreamingService
vocals-sd:StreamingService rdf:type owl:Class ;
                           rdfs:comment "An instance of vois-sd:StreamingService represents a streaming service made available via a certain streaming protocol." .


###  https://w3id.org/rsp/vocals-sd#TimeBasedWindow
vocals-sd:TimeBasedWindow rdf:type owl:Class ;
                          rdfs:subClassOf vocals-sd:Window ;
                          rdfs:comment "A time-based window is a window defined through two time instants o, c (respectively named opening and closing time instants) such that: W(S) = {d|(d, t) ∈ S ∧ t ∈ (o, c]}" .


###  https://w3id.org/rsp/vocals-sd#TimeControl
vocals-sd:TimeControl rdf:type owl:Class ;
                      rdfs:subClassOf vocals-sd:RSPFeature .


###  https://w3id.org/rsp/vocals-sd#TimeSemantics
vocals-sd:TimeSemantics rdf:type owl:Class ;
                        rdfs:subClassOf vocals-sd:RSPFeature .


###  https://w3id.org/rsp/vocals-sd#TimeVaryingGraph
vocals-sd:TimeVaryingGraph rdf:type owl:Class ;
                           rdfs:comment "A time-varying graph G is a function that relates time instants t ∈ T to RDF graphs: G : T → {g | g is an RDF graph}" .


###  https://w3id.org/rsp/vocals-sd#Window
vocals-sd:Window rdf:type owl:Class ;
                 rdfs:subClassOf <http://www.w3.org/ns/dcat#Dataset> ;
                 rdfs:comment "A window W(S) is a set of RDF statements extracted from a stream S." .


#################################################################
#    Individuals
#################################################################

###  http://www.w3.org/ns/sparql-service-description#BasicFederatedQuery
sd:BasicFederatedQuery rdf:type owl:NamedIndividual ,
                                sd:Feature ;
                       rdfs:comment "sd:BasicFederatedQuery, when used as the object of the sd:feature property, indicates that the SPARQL service supports basic federated query using the SERVICE keyword as defined by SPARQL 1.1 Federation Extensions." ;
                       rdfs:label "Basic Federated Query" .


###  http://www.w3.org/ns/sparql-service-description#DereferencesURIs
sd:DereferencesURIs rdf:type owl:NamedIndividual ,
                             sd:Feature ;
                    rdfs:comment "sd:DereferencesURIs, when used as the object of the sd:feature property, indicates that a SPARQL service will dereference URIs used in FROM/FROM NAMED and USING/USING NAMED clauses and use the resulting RDF in the dataset during query evaluation." ;
                    rdfs:label "Dereferences URIs" .


###  http://www.w3.org/ns/sparql-service-description#EmptyGraphs
sd:EmptyGraphs rdf:type owl:NamedIndividual ,
                        sd:Feature ;
               rdfs:comment "sd:EmptyGraphs, when used as the object of the sd:feature property, indicates that the underlying graph store supports empty graphs. A graph store that supports empty graphs MUST NOT remove graphs that are left empty after triples are removed from them." ;
               rdfs:label "Empty Graphs" .


###  http://www.w3.org/ns/sparql-service-description#RequiresDataset
sd:RequiresDataset rdf:type owl:NamedIndividual ,
                            sd:Feature ;
                   rdfs:comment "sd:RequiresDataset, when used as the object of the sd:feature property, indicates that the SPARQL service requires an explicit dataset declaration (based on either FROM/FROM NAMED clauses in a query, USING/USING NAMED clauses in an update, or the appropriate SPARQL Protocol parameters)." ;
                   rdfs:label "Requires Dataset" .


###  http://www.w3.org/ns/sparql-service-description#SPARQL10Query
sd:SPARQL10Query rdf:type owl:NamedIndividual ,
                          sd:Language ;
                 rdfs:comment "sd:SPARQL10Query is an sd:Language representing the SPARQL 1.0 Query language." ;
                 rdfs:label "SPARQL 1.0 Query" .


###  http://www.w3.org/ns/sparql-service-description#SPARQL11Query
sd:SPARQL11Query rdf:type owl:NamedIndividual ,
                          sd:Language ;
                 rdfs:comment "sd:SPARQL11Query is an sd:Language representing the SPARQL 1.1 Query language." ;
                 rdfs:label "SPARQL 1.1 Query" .


###  http://www.w3.org/ns/sparql-service-description#SPARQL11Update
sd:SPARQL11Update rdf:type owl:NamedIndividual ,
                           sd:Language ;
                  rdfs:comment "sd:SPARQLUpdate is an sd:Language representing the SPARQL 1.1 Update language." ;
                  rdfs:label "SPARQL 1.1 Update" .


###  http://www.w3.org/ns/sparql-service-description#UnionDefaultGraph
sd:UnionDefaultGraph rdf:type owl:NamedIndividual ,
                              sd:Feature ;
                     rdfs:comment "sd:UnionDefaultGraph, when used as the object of the sd:feature property, indicates that the default graph of the dataset used during query and update evaluation (when an explicit dataset is not specified) is comprised of the union of all the named graphs in that dataset." ;
                     rdfs:label "Union Default Graph" .


###  https://w3id.org/rsp/vocals-sd#RSPQL
vocals-sd:RSPQL rdf:type owl:NamedIndividual ,
                         sd:Language .


###  https://w3id.org/rsp/vocals-sd#difference
vocals-sd:difference rdf:type owl:NamedIndividual ,
                              vocals-sd:SetOperation .


###  https://w3id.org/rsp/vocals-sd#event_time
vocals-sd:event_time rdf:type owl:NamedIndividual ,
                              vocals-sd:TimeSemantics .


###  https://w3id.org/rsp/vocals-sd#external_time_control
vocals-sd:external_time_control rdf:type owl:NamedIndividual ,
                                         vocals-sd:TimeControl .


###  https://w3id.org/rsp/vocals-sd#filtering
vocals-sd:filtering rdf:type owl:NamedIndividual ,
                             vocals-sd:S2SOperation .


###  https://w3id.org/rsp/vocals-sd#ingestion_time
vocals-sd:ingestion_time rdf:type owl:NamedIndividual ,
                                  vocals-sd:TimeSemantics .


###  https://w3id.org/rsp/vocals-sd#internal_time_control
vocals-sd:internal_time_control rdf:type owl:NamedIndividual ,
                                         vocals-sd:TimeControl .


###  https://w3id.org/rsp/vocals-sd#intersection
vocals-sd:intersection rdf:type owl:NamedIndividual ,
                                vocals-sd:SetOperation .


###  https://w3id.org/rsp/vocals-sd#non_empty_content
vocals-sd:non_empty_content rdf:type owl:NamedIndividual ,
                                     vocals-sd:ReportingPolicy .


###  https://w3id.org/rsp/vocals-sd#on_content_change
vocals-sd:on_content_change rdf:type owl:NamedIndividual ,
                                     vocals-sd:ReportingPolicy .


###  https://w3id.org/rsp/vocals-sd#on_window_close
vocals-sd:on_window_close rdf:type owl:NamedIndividual ,
                                   vocals-sd:ReportingPolicy .


###  https://w3id.org/rsp/vocals-sd#periodic
vocals-sd:periodic rdf:type owl:NamedIndividual ,
                            vocals-sd:ReportingPolicy .


###  https://w3id.org/rsp/vocals-sd#processing_time
vocals-sd:processing_time rdf:type owl:NamedIndividual ,
                                   vocals-sd:TimeSemantics .


###  https://w3id.org/rsp/vocals-sd#replaying
vocals-sd:replaying rdf:type owl:NamedIndividual ,
                             vocals-sd:R2SOperation .


###  https://w3id.org/rsp/vocals-sd#union
vocals-sd:union rdf:type owl:NamedIndividual ,
                         vocals-sd:SetOperation .


###  https://w3id.org/rsp/vocals-sd#windowing
vocals-sd:windowing rdf:type owl:NamedIndividual ,
                             vocals-sd:S2ROperation .


#################################################################
#    General axioms
#################################################################

[ rdf:type owl:AllDisjointClasses ;
  owl:members ( vocals-sd:CatalogService
                vocals-sd:ProcessingService
                vocals-sd:PublishingService
              )
] .


###  Generated by the OWL API (version 4.2.8.20170104-2310) https://github.com/owlcs/owlapi
