@prefix : <https://w3id.org/rsp/vocals-sd#> .
@prefix dc: <http://purl.org/dc/elements/1.1/> .
@prefix sd: <http://www.w3.org/ns/sparql-service-description#> .
@prefix owl: <http://www.w3.org/2002/07/owl#> .
@prefix rdf: <http://www.w3.org/1999/02/22-rdf-syntax-ns#> .
@prefix xml: <http://www.w3.org/XML/1998/namespace> .
@prefix xsd: <http://www.w3.org/2001/XMLSchema#> .
@prefix frmt: <http://www.w3.org/ns/formats/> .
@prefix rdfs: <http://www.w3.org/2000/01/rdf-schema#> .
@prefix time: <http://www.w3.org/2006/time#> .
@prefix vann: <http://purl.org/vocab/vann/> .
@prefix vprov: <https://w3id.org/rsp/vocals-prov#> .
@prefix vocals: <https://w3id.org/rsp/vocals#> .
@prefix dcterms: <http://purl.org/dc/terms/> .

<https://w3id.org/rsp/vocals-sd> a owl:Ontology ;
                               <http://purl.org/dc/elements/1.1/publisher> <http://aislab.hevs.ch/> ;
                               <http://purl.org/dc/terms/description> "Esta ontología has sido diseñada para representar Streams de datos en RDF, así como los endpoints a través de los cuales se puede acceder a los datos de estos streams;  y los meta datos correspondientes."@es ;
                               <http://purl.org/dc/terms/modified> "2017-12-30"^^xsd:date ;
                               <http://purl.org/dc/terms/rights> "Copyright © 2017 Politecnico di Milano & HES-SO Valais-Wallis"^^xsd:string ;
                               <http://purl.org/dc/terms/issued> "2017-12-29"^^xsd:date ;
                               <http://purl.org/dc/terms/license> <https://creativecommons.org/licenses/by/4.0/> ;
                               <http://purl.org/dc/terms/publisher> <http://w3id.org/hes-so/aislab> ;
                               <http://purl.org/dc/terms/title> "VoCaLS: A Vocabulary and Catalog for Linked Streams"@en ;
                               <http://purl.org/dc/terms/description> "This ontology aims to model RDF streams, their metadata, and access endpoints for publishing and consuming these streams"@en ;
                               <http://purl.org/dc/terms/title> "VoCaLS: Vocabulario y catálogo para Streams enlazados"@es ;
                               rdfs:comment "Esta ontología has sido diseñada para representar Streams de datos en RDF, así como los endpoints a través de los cuales se puede acceder a los datos de estos streams;  y los meta datos correspondientes."@es ;
                               owl:versionInfo "0.1.1"^^xsd:string ;
                               rdfs:comment "This ontology aims to model RDF streams, their metadata, and access endpoints for publishing and consuming these streams"@en ;
                               <http://purl.org/dc/terms/title> "VoCaLS: ontologie de representation de données et metadonnées de streams"@fr ;
                               rdfs:comment "Cette ontologie a été conçue pour representer des données et meta-données de streams RDF, ainsi que leurs points d'accès."@fr ;
                               <http://purl.org/dc/terms/description> "Cette ontologie a été conçue pour representer des données et meta-données de streams RDF, ainsi que leurs points d'accès."@fr .	owl:versionIRI <https://w3id.org/rsp/vocals-sd> ;
	vann:preferredNamespaceUri "https://w3id.org/rsp/vocals-sd#" ;
	dc:creator vocals:RiccardoTommasini ;
	vann:preferredNamespacePrefix "vocals-sd" ;
	dc:creator <http://w3id.org/people/jpcik/me> ;
	dcterms:created "2017-12-23T13:00:00"^^xsd:dateTime ;
	dc:creator vocals:YehiaAboSedira .

# 
# 
# #################################################################
# #
# #    Annotation properties
# #
# #################################################################
# 
# 
# https://w3id.org/rsp/vocals-sd#name

:name a owl:AnnotationProperty ;
	rdfs:comment "Relates a named time varying graph to the name by which it may be referenced in a FROM/FROM NAMED clause. The object of the vsd:name property is an IRI." ;
	rdfs:domain :TimeVaryingGraph .
# 
# 
# 
# #################################################################
# #
# #    Object Properties
# #
# #################################################################
# 
# 
# https://w3id.org/rsp/vocals-sd#availableGraphs

:availableGraphs a owl:ObjectProperty ;
	rdfs:domain :RDFStreamService ;
	rdfs:range :TimeVaryingGraph ;
	rdfs:comment "Relates an instance of vsd:RSService to the time varying graphs available by the vsd:RSService." .
# 
# https://w3id.org/rsp/vocals-sd#availableStream

:availableStream a owl:ObjectProperty ;
	rdfs:subPropertyOf owl:topObjectProperty ;
	rdfs:domain :RDFStreamService ;
	rdfs:range vocals:RDFStream .
# 
# https://w3id.org/rsp/vocals-sd#defaultGraph

:defaultGraph a owl:ObjectProperty ;
	rdfs:domain :SDS ;
	rdfs:range :TimeVaryingGraph ;
	rdfs:comment "Relates an instance of vocals:RDFStream to the description of its default graph." .
# 
# https://w3id.org/rsp/vocals-sd#defaultSDS

:defaultSDS a owl:ObjectProperty ;
	rdfs:domain :RDFStreamService ;
	rdfs:range :SDS ;
	rdfs:comment "Relates an instance of vsd:RSService to a description of the default SDS available when no explicit dataset is specified in the query." .
# 
# https://w3id.org/rsp/vocals-sd#describedBy

:describedBy a owl:ObjectProperty ;
	rdfs:domain vocals:RDFStream ;
	rdfs:range :CatalogService ;
	rdfs:comment "Points to an instance of vsd:CatalogingService that describes a certain vocals:RDFStream." .
# 
# https://w3id.org/rsp/vocals-sd#endedAt

:endedAt a owl:ObjectProperty ;
	rdfs:domain :Window ;
	rdfs:range time:Instant .
# 
# https://w3id.org/rsp/vocals-sd#graph

:graph a owl:ObjectProperty ;
	rdfs:range :TimeVaryingGraph ;
	rdfs:comment "Relates a named time varying graph to its graph description." .
# 
# https://w3id.org/rsp/vocals-sd#hasFeature

:hasFeature a owl:ObjectProperty ;
	rdfs:domain :RDFStreamService ;
	rdfs:range :RDFStreamingFeature ;
	rdfs:comment "Relates a vsd:RSService to an available feature" .
# 
# https://w3id.org/rsp/vocals-sd#namedTimeVaryingGraph

:namedTimeVaryingGraph a owl:ObjectProperty ;
	rdfs:domain :SDS ;
	rdfs:range :TimeVaryingGraph ;
	rdfs:comment "Relates an instance of vocals:SDS to the description of one of its named time varying graphs. The description of such a named time varying graph MUST include the vsd:name property." .
# 
# https://w3id.org/rsp/vocals-sd#publishedBy

:publishedBy a owl:ObjectProperty ;
	rdfs:domain vocals:RDFStream ;
	rdfs:range :PublishingService ;
	rdfs:comment "Points to an instance of vsd:PublishingService that publishs a certain vocals:RDFStream." .
# 
# https://w3id.org/rsp/vocals-sd#registerdTask

:registerdTask a owl:ObjectProperty ;
	rdfs:domain :RDFStreamService ;
	rdfs:comment "Relates an instance of vsd:RSService with instances of running tasks, e.g. RSP-QL Query ." ;
	rdfs:label "registerd task" .
# 
# https://w3id.org/rsp/vocals-sd#registeredBy

:registeredBy a owl:ObjectProperty ;
	rdfs:domain vocals:RDFStream ;
	rdfs:range :ProcessingService ;
	rdfs:comment "Points to an instance of vsd:ProcessingService that registers/ processes a certain vocals:RDFStream." .
# 
# https://w3id.org/rsp/vocals-sd#registeredStreams

:registeredStreams a owl:ObjectProperty ;
	rdfs:domain :RDFStreamService ;
	rdfs:range vocals:RDFStream ;
	rdfs:comment "Relates an instance of vsd:RSService to the streams registered on it." .
# 
# https://w3id.org/rsp/vocals-sd#resultFormat

:resultFormat a owl:ObjectProperty ;
	rdfs:domain :RDFStreamService ;
	rdfs:range frmt:Format ;
	rdfs:comment "Relates an instance of sd:Service to a format that is supported for serializing query results." ;
	rdfs:label "result format" .
# 
# https://w3id.org/rsp/vocals-sd#rspEndpoint

:rspEndpoint a owl:ObjectProperty ;
	rdfs:domain :RDFStreamService ;
	rdfs:comment "The RSP-QL endpoint of an vocals:RSPService that implements the RSP-QL Protocol service. The object of the vocals:rspEndpoint property is an IRI." ;
	rdfs:label "RSP endpoint" .
# 
# https://w3id.org/rsp/vocals-sd#startedAt

:startedAt a owl:ObjectProperty ;
	rdfs:domain :Window ;
	rdfs:range time:Instant .
# 
# 
# 
# #################################################################
# #
# #    Classes
# #
# #################################################################
# 
# 
# http://www.w3.org/2006/time#Instant

time:Instant a owl:Class .
# 
# http://www.w3.org/ns/dcat#Dataset

<http://www.w3.org/ns/dcat#Dataset> a owl:Class .
# 
# http://www.w3.org/ns/formats/Format

frmt:Format a owl:Class .
# 
# https://w3id.org/rsp/vocals#RDFStream

vocals:RDFStream a owl:Class .
# 
# https://w3id.org/rsp/vocals-sd#CatalogService

:CatalogService a owl:Class ;
	rdfs:subClassOf :RDFStreamService ;
	rdfs:comment "An vsd:CatalogService is a service storing stream descriptions. (e.g. SPARQL endpoint, RDF file with stream description,...etc)" ;
	rdfs:label "Catalog service" ;
	rdfs:seeAlso "vocals:StreamDescriptor" .
# 
# https://w3id.org/rsp/vocals-sd#Operation

:Operation a owl:Class ;
	rdfs:subClassOf :RDFStreamingFeature ;
	rdfs:comment "An operation represents an available action/function that can be performed by an RDF Stream Service. An operation may ingest stream items or static data items, and output either of them."@en ;
	rdfs:label "Operation"@en .
# 
# https://w3id.org/rsp/vocals-sd#PhysicalWindow

:PhysicalWindow a owl:Class ;
	rdfs:subClassOf :Window ;
	rdfs:comment "Window defined by an interval size (in units of RDF elements)" .
# 
# https://w3id.org/rsp/vocals-sd#ProcessingService

:ProcessingService a owl:Class ;
	rdfs:subClassOf :RDFStreamService ;
	rdfs:comment "An vsd:ProcessingService represents an RDF stream processing service. Processing means any kind of transformation on streaming data, i.e., Querying, Reasoning, Filtering...etc" .
# 
# https://w3id.org/rsp/vocals-sd#PublishingService

:PublishingService a owl:Class ;
	rdfs:subClassOf :RDFStreamService ;
	rdfs:comment "An vsd:PublishingService represents a stream publishing service. Publishing has to be interpreted as in Linked Data domain, where is possible." .
# 
# https://w3id.org/rsp/vocals-sd#R2ROperation

:R2ROperation a owl:Class ;
	rdfs:subClassOf :Operation ;
	rdfs:comment "An R2ROperation represents a realtion-to-relation operation that an RDF Stream Service can perform, such as filtering, aggregation, projection, join, etc. It takes as input a relation (e.g. RDF data mappings) and outputs also a relation (e.g. RDF data mappings)."@en ;
	rdfs:label "Relation-to-Relation Operation"@en .
# 
# https://w3id.org/rsp/vocals-sd#R2SOperation

:R2SOperation a owl:Class ;
	rdfs:subClassOf :Operation ;
	rdfs:comment "An R2SOperation represents a realtion-to-stream operation that an RDF Stream Service can perform. It takes as input a relation (e.g. RDF data mappings), and ouputs RDF Stream elements, e.g. for instance an operation that replays a static dataset as a stream, or an Istream, Rstream or Dstream operation."@en ;
	rdfs:label "Relation-to-Stream operation"@en .
# 
# https://w3id.org/rsp/vocals-sd#RDFStreamService

:RDFStreamService a owl:Class ;
	rdfs:subClassOf :StreamingService ;
	rdfs:comment "An instance of vsd:Service represents a RDF streaming service made available via RDF streaming protocol." ;
	rdfs:label "RDF stream service" .
# 
# https://w3id.org/rsp/vocals-sd#RDFStreamingFeature

:RDFStreamingFeature a owl:Class ;
	rdfs:comment "Represents a feature of a RDF Streaming service. Features may include operations over RDF streams, policies, time handling mechanisms, etc."@en ;
	rdfs:label "RDF Streaming Feature"@en .
# 
# https://w3id.org/rsp/vocals-sd#ReportingPolicy

:ReportingPolicy a owl:Class ;
	rdfs:subClassOf :RDFStreamingFeature ;
	rdfs:label "Reporting Policy" .
# 
# https://w3id.org/rsp/vocals-sd#S2ROperation

:S2ROperation a owl:Class ;
	rdfs:subClassOf :Operation ;
	rdfs:comment "An instance of vsd:R2ROperation represent a stream-to-relation operation that an vsd:RSService can perform. (e.g. windowing)" ;
	rdfs:label "stream-to-relation operation" .
# 
# https://w3id.org/rsp/vocals-sd#S2SOperation

:S2SOperation a owl:Class ;
	rdfs:subClassOf :Operation ;
	rdfs:comment "An instance of vsd:R2ROperation represent a stream-to-stream operation that an vsd:RSService can perform. (e.g. transformation)" ;
	rdfs:label "stream-to-stream operation" .
# 
# https://w3id.org/rsp/vocals-sd#SDS

:SDS a owl:Class ;
	rdfs:comment "A streaming dataset is a set composed by an (optional) default graph, n (n ≥ 0) named graphs and m (m ≥ 0) named time-varying graphs" ;
	rdfs:label "SDS" .
# 
# https://w3id.org/rsp/vocals-sd#SetOperation

:SetOperation a owl:Class ;
	rdfs:subClassOf :S2SOperation ;
	rdfs:comment "An instance of vsd:SetOperation represents an available set operator that can be performed by vsd:RSService. (e.g. union, intersection)" ;
	rdfs:label "Set operation" .
# 
# https://w3id.org/rsp/vocals-sd#StreamingService

:StreamingService a owl:Class ;
	rdfs:comment "An instance of vsd:StreamingService represents a streaming service made available via a certain streaming protocol." ;
	rdfs:label "Streaming service" .
# 
# https://w3id.org/rsp/vocals-sd#TimeBasedWindow

:TimeBasedWindow a owl:Class ;
	rdfs:subClassOf :Window ;
	rdfs:comment "A time-based window is a window defined through two time instants o, c (respectively named opening and closing time instants) such that: W(S) = {d|(d, t) ∈ S ∧ t ∈ (o, c]}" .
# 
# https://w3id.org/rsp/vocals-sd#TimeControl

:TimeControl a owl:Class ;
	rdfs:subClassOf :RDFStreamingFeature .
# 
# https://w3id.org/rsp/vocals-sd#TimeSemantics

:TimeSemantics a owl:Class ;
	rdfs:subClassOf :RDFStreamingFeature .
# 
# https://w3id.org/rsp/vocals-sd#TimeVaryingGraph

:TimeVaryingGraph a owl:Class ;
	rdfs:comment "A time-varying graph G is a function that relates time instants t ∈ T to RDF graphs: G : T → {g | g is an RDF graph}" .
# 
# https://w3id.org/rsp/vocals-sd#Window

:Window a owl:Class ;
	rdfs:subClassOf <http://www.w3.org/ns/dcat#Dataset> ;
	rdfs:comment "A window W(S) is a set of RDF statements extracted from a stream S." .
# 
# 
# 
# #################################################################
# #
# #    Individuals
# #
# #################################################################
# 
# 
# https://w3id.org/rsp/vocals-sd#RSPQL

:RSPQL a owl:NamedIndividual , :S2SOperation .
# 
# https://w3id.org/rsp/vocals-sd#count

:count a owl:NamedIndividual , :R2ROperation .
# 
# https://w3id.org/rsp/vocals-sd#difference

:difference a owl:NamedIndividual , :SetOperation .
# 
# https://w3id.org/rsp/vocals-sd#event_time

:event_time a owl:NamedIndividual , :TimeSemantics .
# 
# https://w3id.org/rsp/vocals-sd#external_time_control

:external_time_control a owl:NamedIndividual , :TimeControl .
# 
# https://w3id.org/rsp/vocals-sd#filtering

:filtering a owl:NamedIndividual , :S2SOperation .
# 
# https://w3id.org/rsp/vocals-sd#ingestion_time

:ingestion_time a owl:NamedIndividual , :TimeSemantics .
# 
# https://w3id.org/rsp/vocals-sd#internal_time_control

:internal_time_control a owl:NamedIndividual , :TimeControl .
# 
# https://w3id.org/rsp/vocals-sd#intersection

:intersection a owl:NamedIndividual , :SetOperation .
# 
# https://w3id.org/rsp/vocals-sd#non_empty_content

:non_empty_content a owl:NamedIndividual , :ReportingPolicy .
# 
# https://w3id.org/rsp/vocals-sd#on_content_change

:on_content_change a owl:NamedIndividual , :ReportingPolicy .
# 
# https://w3id.org/rsp/vocals-sd#on_window_close

:on_window_close a owl:NamedIndividual , :ReportingPolicy .
# 
# https://w3id.org/rsp/vocals-sd#periodic

:periodic a owl:NamedIndividual , :ReportingPolicy .
# 
# https://w3id.org/rsp/vocals-sd#processing_time

:processing_time a owl:NamedIndividual , :TimeSemantics .
# 
# https://w3id.org/rsp/vocals-sd#replaying

:replaying a owl:NamedIndividual , :R2SOperation .
# 
# https://w3id.org/rsp/vocals-sd#sum

:sum a owl:NamedIndividual , :R2ROperation .
# 
# https://w3id.org/rsp/vocals-sd#transform

:transform a owl:NamedIndividual , :S2SOperation .
# 
# https://w3id.org/rsp/vocals-sd#union

:union a owl:NamedIndividual , :SetOperation .
# 
# https://w3id.org/rsp/vocals-sd#windowing

:windowing a owl:NamedIndividual , :S2ROperation .
# 
# Generated by the OWL API (version 4.2.5.20160517-0735) https://github.com/owlcs/owlapi
