@prefix : <https://w3id.org/rsp/vocals-prov#> .
@prefix dc: <http://purl.org/dc/elements/1.1/> .
@prefix owl: <http://www.w3.org/2002/07/owl#> .
@prefix rdf: <http://www.w3.org/1999/02/22-rdf-syntax-ns#> .
@prefix vsd: <https://w3id.org/rsp/vocals-sd#> .
@prefix xml: <http://www.w3.org/XML/1998/namespace> .
@prefix xsd: <http://www.w3.org/2001/XMLSchema#> .
@prefix prov: <http://www.w3.org/ns/prov#> .
@prefix rdfs: <http://www.w3.org/2000/01/rdf-schema#> .
@prefix time: <http://www.w3.org/2006/time#> .
@prefix vann: <http://purl.org/vocab/vann/> .
@prefix vocals: <https://w3id.org/rsp/vocals#> .
@prefix dcterms: <http://purl.org/dc/terms/> .

<https://w3id.org/rsp/vocals-prov> a owl:Ontology ;
	owl:versionIRI <https://w3id.org/rsp/vocals-prov> ;
	dc:publisher <http://aislab.hevs.ch/> ;
	dc:creator vocals:RiccardoTommasini ;
	dcterms:modified "2017-12-30"^^xsd:date ;
	dc:creator <http://w3id.org/people/jpcik/me> ;
	dcterms:rights "Copyright © 2017 Politecnico di Milano & HES-SO Valais-Wallis"^^xsd:string ;
	dcterms:description "Cette ontologie a été conçue pour representer la provenance de données et meta-données de streams RDF, ainsi que leurs points d'accès."@fr ;
	dcterms:title "VoCaLS-Prov: Vocabulario y catálogo para Streams enlazados, módulo de Provenance"@es ;
	vann:preferredNamespaceUri "https://w3id.org/rsp/vocals-prov#" ;
	dcterms:title "VoCaLS-Prov: A Vocabulary and Catalog for Linked Streams, Provenance Module"@en ;
	dcterms:description "Esta ontología has sido diseñada para representar provenance de Streams de datos en RDF, así como los endpoints a través de los cuales se puede acceder a los datos de estos streams;  y los meta datos correspondientes."@es ;
	rdfs:comment "Cette ontologie a été conçue pour representer la provenance de données et meta-données de streams RDF, ainsi que leurs points d'accès."@fr , "Esta ontología has sido diseñada para representar provenance de Streams de datos en RDF, así como los endpoints a través de los cuales se puede acceder a los datos de estos streams;  y los meta datos correspondientes."@es ;
	dcterms:license <https://creativecommons.org/licenses/by/4.0/> ;
	dcterms:publisher <http://w3id.org/hes-so/aislab> ;
	dcterms:created "2017-12-23T13:00:00"^^xsd:dateTime ;
	dcterms:issued "2017-12-29"^^xsd:date ;
	rdfs:comment "This ontology aims to model provenance of RDF streams, their metadata, and access endpoints for publishing and consuming these streams"@en ;
	dc:creator vocals:YehiaAboSedira ;
	dcterms:title "VoCaLS-Prov: ontologie de representation de provenance pour données et metadonnées de streams RDF"@fr ;
	vann:preferredNamespacePrefix "vocals-prov" ;
	owl:versionInfo "0.1.1"^^xsd:string ;
	dcterms:description "This ontology aims to model provenance of RDF streams, their metadata, and access endpoints for publishing and consuming these streams"@en .
# 
# 
# #################################################################
# #
# #    Object Properties
# #
# #################################################################
# 
# 
# https://w3id.org/rsp/vocals-prov#containedIn

:containedIn a owl:ObjectProperty ;
	owl:inverseOf :contains ;
	rdfs:domain :Operator ;
	rdfs:range :Task ;
	rdfs:comment "Relates an Operator to the containing Task."@en ;
	rdfs:label "containedIn"@en .
# 
# https://w3id.org/rsp/vocals-prov#contains

:contains a owl:ObjectProperty ;
	rdfs:domain :Task ;
	rdfs:range :Operator ;
	rdfs:comment "Relates a Task to Operator used to finish the task."@en ;
	rdfs:label "contains"@en .
# 
# https://w3id.org/rsp/vocals-prov#endedAt

:endedAt a owl:ObjectProperty ;
	rdfs:domain :Window ;
	rdfs:range time:Instant .
# 
# https://w3id.org/rsp/vocals-prov#followedBy

:followedBy a owl:ObjectProperty ;
	owl:inverseOf :precededBy ;
	rdfs:domain :Operator ;
	rdfs:range :Operator ;
	rdfs:comment "Points to the following :operator to be applied after the current one in a :Task." .
# 
# https://w3id.org/rsp/vocals-prov#hasOutput

:hasOutput a owl:ObjectProperty ;
	rdfs:domain :Task ;
	rdfs:range prov:Entity ;
	rdfs:comment "Points to the output of a :operator to be applied before the current one in a :Task." .
# 
# https://w3id.org/rsp/vocals-prov#performs

:performs a owl:ObjectProperty ;
	rdfs:range vsd:Operation ;
	rdfs:isDefinedBy "Relate vsd:Operation to :Operator ." .
# 
# https://w3id.org/rsp/vocals-prov#precededBy

:precededBy a owl:ObjectProperty ;
	rdfs:domain :Operator ;
	rdfs:range :Operator ;
	rdfs:comment "Points to the preceding :operator to be applied before the current one in a :Task." .
# 
# https://w3id.org/rsp/vocals-prov#startedAt

:startedAt a owl:ObjectProperty ;
	rdfs:domain :Window ;
	rdfs:range time:Instant .
# 
# https://w3id.org/rsp/vocals-prov#startingTime

:startingTime a owl:ObjectProperty ;
	rdfs:domain :WindowOperator ;
	rdfs:range time:Instant .
# 
# 
# 
# #################################################################
# #
# #    Data properties
# #
# #################################################################
# 
# 
# https://w3id.org/rsp/vocals-prov#query

:query a owl:DatatypeProperty ;
	rdfs:subPropertyOf owl:topDataProperty ;
	rdfs:domain :RSPQLOperator .
# 
# https://w3id.org/rsp/vocals-prov#range

:range a owl:DatatypeProperty ;
	rdfs:subPropertyOf owl:topDataProperty ;
	rdfs:domain :WindowOperator .
# 
# https://w3id.org/rsp/vocals-prov#step

:step a owl:DatatypeProperty ;
	rdfs:subPropertyOf owl:topDataProperty ;
	rdfs:domain :WindowOperator .
# 
# 
# 
# #################################################################
# #
# #    Classes
# #
# #################################################################
# 
# 
# http://www.w3.org/2006/time#Instant

time:Instant a owl:Class .
# 
# http://www.w3.org/ns/dcat#Dataset

<http://www.w3.org/ns/dcat#Dataset> a owl:Class .
# 
# http://www.w3.org/ns/prov#Activity

prov:Activity a owl:Class .
# 
# http://www.w3.org/ns/prov#Entity

prov:Entity a owl:Class .
# 
# http://www.w3.org/ns/prov#SoftwareAgent

prov:SoftwareAgent a owl:Class .
# 
# https://w3id.org/rsp/vocals-prov#FilterOperator

:FilterOperator a owl:Class ;
	rdfs:subClassOf :S2SOperator ;
	rdfs:comment "A :FilterOperator represents an operator that exclude data that doesn't match some specified criteria." .
# 
# https://w3id.org/rsp/vocals-prov#Operator

:Operator a owl:Class ;
	rdfs:subClassOf prov:Activity ;
	rdfs:comment "Operator that operat on an entity to generate another entity." .
# 
# https://w3id.org/rsp/vocals-prov#PhysicalWindow

:PhysicalWindow a owl:Class ;
	rdfs:subClassOf :Window ;
	rdfs:comment "Window defined by an interval size (in units of RDF elements)" .
# 
# https://w3id.org/rsp/vocals-prov#R2ROperator

:R2ROperator a owl:Class ;
	rdfs:subClassOf :Operator ;
	rdfs:comment "Operators that produce relations from other relations." ;
	rdfs:isDefinedBy "Arvind Arasu, Shivnath Babu, and Jennifer Widom. 2006. The CQL continuous query language: semantic foundations and query execution. The VLDB Journal 15, 2 (June 2006), 121-142. DOI=http://dx.doi.org/10.1007/s00778-004-0147-z" .
# 
# https://w3id.org/rsp/vocals-prov#R2SOperator

:R2SOperator a owl:Class ;
	rdfs:subClassOf :Operator ;
	rdfs:comment "Operators that produce a stream from a relation." ;
	rdfs:isDefinedBy "Arvind Arasu, Shivnath Babu, and Jennifer Widom. 2006. The CQL continuous query language: semantic foundations and query execution. The VLDB Journal 15, 2 (June 2006), 121-142. DOI=http://dx.doi.org/10.1007/s00778-004-0147-z" .
# 
# https://w3id.org/rsp/vocals-prov#RSPQLOperator

:RSPQLOperator a owl:Class ;
	rdfs:subClassOf :S2SOperator ;
	owl:disjointWith :SetOperator ;
	rdfs:comment "RDF Stream Processing (RSP) Operators that produce a stream by appling a C-Sparql query to another stream." .
# 
# https://w3id.org/rsp/vocals-prov#Replay

:Replay a owl:Class ;
	rdfs:subClassOf :R2SOperator ;
	rdfs:comment "Replay operator produce a stream from a static RDF dataset" ;
	rdfs:isDefinedBy "https://link.springer.com/chapter/10.1007%2F978-3-319-46547-0_15" .
# 
# https://w3id.org/rsp/vocals-prov#S2ROperator

:S2ROperator a owl:Class ;
	rdfs:subClassOf :Operator ;
	rdfs:comment "Operators that produce a relation from a stream." ;
	rdfs:isDefinedBy "Arvind Arasu, Shivnath Babu, and Jennifer Widom. 2006. The CQL continuous query language: semantic foundations and query execution. The VLDB Journal 15, 2 (June 2006), 121-142. DOI=http://dx.doi.org/10.1007/s00778-004-0147-z" .
# 
# https://w3id.org/rsp/vocals-prov#S2SOperator

:S2SOperator a owl:Class ;
	rdfs:subClassOf :Operator ;
	rdfs:comment "Operators that produce a stream form another stream." .
# 
# https://w3id.org/rsp/vocals-prov#SetOperator

:SetOperator a owl:Class ;
	rdfs:subClassOf :S2SOperator ;
	rdfs:comment "Operator that produce a stream by applying set algebra operator on other streams." .
# 
# https://w3id.org/rsp/vocals-prov#StreamingAgent

:StreamingAgent a owl:Class ;
	rdfs:subClassOf prov:SoftwareAgent ;
	rdfs:comment "An instance of a :StreamingAgent represent an actor that applies an :Operator that consums and/or produce a stream." ;
	rdfs:label "StreamingAgent"@en .
# 
# https://w3id.org/rsp/vocals-prov#Task

:Task a owl:Class ;
	rdfs:comment "A task contains one or more activity to be applied on a prov:Entity." .
# 
# https://w3id.org/rsp/vocals-prov#TimeBasedWindow

:TimeBasedWindow a owl:Class ;
	rdfs:subClassOf :Window ;
	rdfs:comment "A time-based window is a window defined through two time instants o, c (respectively named opening and closing time instants) such that: W(S) = {d|(d, t) ∈ S ∧ t ∈ (o, c]}" .
# 
# https://w3id.org/rsp/vocals-prov#TransformOperator

:TransformOperator a owl:Class ;
	rdfs:subClassOf :S2SOperator ;
	rdfs:comment "An instance of :TransformOperator represent an operator that convert a stream from one form to another. (e.g. Convert a raw stream to and RDF stream)" .
# 
# https://w3id.org/rsp/vocals-prov#Window

:Window a owl:Class ;
	rdfs:subClassOf <http://www.w3.org/ns/dcat#Dataset> ;
	rdfs:comment "A window W(S) is a set of RDF statements extracted from a stream S." .
# 
# https://w3id.org/rsp/vocals-prov#WindowOperator

:WindowOperator a owl:Class ;
	rdfs:subClassOf :S2ROperator .
# 
# https://w3id.org/rsp/vocals-sd#Operation

vsd:Operation a owl:Class .
# 
# 
# 
# #################################################################
# #
# #    Individuals
# #
# #################################################################
# 
# 
# https://w3id.org/rsp/vocals-prov#TripleWave

:TripleWave a owl:NamedIndividual , :StreamingAgent .
# 
# https://w3id.org/rsp/vocals-prov#difference_operator

:difference_operator a owl:NamedIndividual , :SetOperator .
# 
# https://w3id.org/rsp/vocals-prov#intersect_operator

:intersect_operator a owl:NamedIndividual , :SetOperator .
# 
# https://w3id.org/rsp/vocals-prov#union_operator

:union_operator a owl:NamedIndividual , :SetOperator .
# 
# Generated by the OWL API (version 4.2.5.20160517-0735) https://github.com/owlcs/owlapi
