@prefix : <http://w3id.org/rsp/vocals#> .
@prefix owl: <http://www.w3.org/2002/07/owl#> .
@prefix rdf: <http://www.w3.org/1999/02/22-rdf-syntax-ns#> .
@prefix xml: <http://www.w3.org/XML/1998/namespace> .
@prefix xsd: <http://www.w3.org/2001/XMLSchema#> .
@prefix dcat: <http://www.w3.org/ns/dcat#> .
@prefix foaf: <http://xmlns.com/foaf/0.1/> .
@prefix rdfs: <http://www.w3.org/2000/01/rdf-schema#> .
@base <http://w3id.org/rsp/vocals#> .

<http://w3id.org/rsp/vocals#> rdf:type owl:Ontology ;
                               owl:imports dcat: ;
                               <http://purl.org/dc/elements/1.1/publisher> <http://aislab.hevs.ch/> ;
                               <http://purl.org/dc/terms/creator> <https://w3id.org/people/rictomm> ;
                               rdfs:comment "This ontology aims to model RDF streams, their metadata, and access endpoints for publishing and consuming these streams"@en ;
                               <http://purl.org/dc/terms/title> "VoCaLS: ontologie de representation de données et metadonnées de streams"@fr ;
                               <http://purl.org/dc/terms/creator> <http://w3id.org/people/jpcik/me> ;
                               <http://purl.org/dc/terms/title> "VoCaLS: A Vocabulary and Catalog for Linked Streams"@en ;
                               <http://purl.org/dc/terms/modified> "2017-12-10"^^xsd:date ;
                               <http://purl.org/dc/terms/rights> "Copyright © 2017 Politecnico di Milano & HES-SO Valais-Wallis"^^xsd:string ;
                               <http://purl.org/vocab/vann/preferredNamespacePrefix> "vocals"^^xsd:string ;
                               <http://purl.org/dc/terms/title> "VoCaLS: Vocabulario y catálogo para Streams enlazados"@es ;
                               <http://purl.org/dc/terms/issued> "2017-12-01"^^xsd:date ;
                               <http://purl.org/vocab/vann/preferredNamespaceUri> "http://w3id.org/rsp/vocals#"^^xsd:string ;
                               rdfs:comment "Esta ontología has sido diseñada para representar Streams de datos en RDF, así como los endpoints a través de los cuales se puede acceder a los datos de estos streams;  y los meta datos correspondientes."@es ;
                               <http://purl.org/dc/terms/license> <https://creativecommons.org/licenses/by/4.0/> ;
                               <http://purl.org/dc/terms/publisher> <http://w3id.org/hes-so/aislab> ;
                               <http://purl.org/dc/terms/description> "This ontology aims to model RDF streams, their metadata, and access endpoints for publishing and consuming these streams"@en ;
                               <http://purl.org/dc/terms/creator> <http://streamreasoning.org/vois#YehiaAboSedira> ;
                               <http://purl.org/dc/terms/description> "Esta ontología has sido diseñada para representar Streams de datos en RDF, así como los endpoints a través de los cuales se puede acceder a los datos de estos streams y los meta datos correspondientes."@es ,
                                                                      "Cette ontologie a été conçue pour representer des données et meta-données de streams RDF, ainsi que leurs points d'accès."@fr ;
                               rdfs:comment "Cette ontologie a été conçue pour representer des données et meta-données de streams RDF, ainsi que leurs points d'accès."@fr ;
                               owl:versionInfo "0.1.1"^^xsd:string .

#################################################################
#    Object Properties
#################################################################

###  http://w3id.org/rsp/vocals#hasEndpoint
:hasEndpoint rdf:type owl:ObjectProperty ;
             rdfs:subPropertyOf dcat:distribution ;
             rdfs:domain :Stream ;
             rdfs:range :StreamEndpoint ;
             rdfs:comment "A relationship between a Stream and a StreamEndpoint. A stream may have several endpoints through which its contents can be accessible."@en ;
             rdfs:isDefinedBy <http://w3id.org/rsp/vocals#> ;
             rdfs:label "hasEndpoint"@en ;
             rdfs:seeAlso :Stream ,
                          :StreamEndpoint .


###  http://w3id.org/rsp/vocals#hasPartition
:hasPartition rdf:type owl:ObjectProperty ;
              rdfs:domain :Stream ;
              rdfs:range :StreamPartition ;
              rdfs:comment "A relationship between a Stream and a partition, or portion of elements streamed"@en ;
              rdfs:isDefinedBy <http://w3id.org/rsp/vocals#> ;
              rdfs:label "hasPartition"@en ;
              rdfs:seeAlso :Stream ,
                           :StreamPartition .


###  http://w3id.org/rsp/vocals#previous
:previous rdf:type owl:ObjectProperty ;
          rdfs:domain :StreamPartition ;
          rdfs:range :StreamPartition ;
          rdfs:comment "Relationship between a stream partition and the previous partition in the stream. it connects stream partitions in order"@en ;
          rdfs:isDefinedBy <http://w3id.org/rsp/vocals#> ;
          rdfs:label "previous"@en ;
          rdfs:seeAlso :StreamPartition .


###  http://w3id.org/rsp/vocals#vocals:stream
:stream rdf:type owl:ObjectProperty ;
        rdfs:subPropertyOf dcat:dataset ;
        rdfs:domain :StreamDescriptor ;
        rdfs:range :Stream .


###  http://www.w3.org/ns/dcat#distribution
dcat:distribution rdf:type owl:ObjectProperty .


#################################################################
#    Classes
#################################################################

###  http://purl.org/vocommons/voaf#Vocabulary
<http://purl.org/vocommons/voaf#Vocabulary> rdf:type owl:Class .


###  http://w3id.org/rsp/vocals#RDFStream
:RDFStream rdf:type owl:Class ;
           rdfs:subClassOf :Stream ;
           rdfs:comment "A stream composed of RDF data elements, i.e. RDF graphs and/or triples."@en ;
           rdfs:isDefinedBy <http://w3id.org/rsp/vocals#> ;
           rdfs:label "RDFStream"@en ;
           rdfs:seeAlso :Stream .


###  http://w3id.org/rsp/vocals#Stream
:Stream rdf:type owl:Class ;
        rdfs:subClassOf dcat:Dataset ;
        rdfs:comment "A potentially infinite sequence of data elements. A stream may be findable and accesible on the Web."@en ;
        rdfs:isDefinedBy <http://w3id.org/rsp/vocals#> ;
        rdfs:label "Stream"@en ;
        rdfs:seeAlso :StreamDistribution .


###  http://w3id.org/rsp/vocals#StreamDescriptor
:StreamDescriptor rdf:type owl:Class ;
                  rdfs:subClassOf dcat:CatalogRecord ,
                                  foaf:Document ;
                  rdfs:comment "A Stream Descriptor is a Web document that contains the description of a Stream."@en ;
                  rdfs:isDefinedBy <http://w3id.org/rsp/vocals#> ;
                  rdfs:label "StreamDescriptor"@en ;
                  rdfs:seeAlso :Stream .


###  http://w3id.org/rsp/vocals#StreamDistribution
:StreamDistribution rdf:type owl:Class ;
                    owl:equivalentClass :StreamEndpoint ;
                    rdfs:subClassOf dcat:Distribution ;
                    rdfs:comment "Represents a specific available form of a stream. Each stream might be available in different forms, these forms might represent different access points of the stream. Examples of distributions include a WebSocket endpoint, an HTTP endpoint, a Server-Sent Events endpoint, MQTT, etc."@en ;
                    rdfs:isDefinedBy <http://w3id.org/rsp/vocals#> ;
                    rdfs:label "StreamDistribution"@en ;
                    rdfs:seeAlso :Stream .


###  http://w3id.org/rsp/vocals#StreamEndpoint
:StreamEndpoint rdf:type owl:Class ;
                rdfs:subClassOf dcat:Distribution ;
                rdfs:comment "Represents a specific available form of a stream. Each stream might be available in different forms, these forms might represent different access points of the stream. Examples of endpoints include a WebSocket endpoint, an HTTP endpoint, a Server-Sent Events endpoint, MQTT, etc."@en ;
                rdfs:isDefinedBy <http://w3id.org/rsp/vocals#> ;
                rdfs:label "StreamEndpoint"@en .


###  http://w3id.org/rsp/vocals#StreamPartition
:StreamPartition rdf:type owl:Class ;
                 rdfs:subClassOf dcat:Dataset ;
                 rdfs:comment "A finite subset of the stream that are made available to be accessed and consumed by standard Linked Data services."@en ;
                 rdfs:isDefinedBy <http://w3id.org/rsp/vocals#> ;
                 rdfs:label "StreamPartition"@en ;
                 rdfs:seeAlso :Stream ,
                              :previous .


###  http://www.w3.org/ns/dcat#CatalogRecord
dcat:CatalogRecord rdf:type owl:Class .


###  http://www.w3.org/ns/dcat#Dataset
dcat:Dataset rdf:type owl:Class .


###  http://www.w3.org/ns/dcat#Distribution
dcat:Distribution rdf:type owl:Class .


###  http://xmlns.com/foaf/0.1/Document
foaf:Document rdf:type owl:Class .


#################################################################
#    Individuals
#################################################################

###  http://w3id.org/rsp/vocals#
<http://w3id.org/rsp/vocals#> rdf:type owl:NamedIndividual ,
                                        <http://purl.org/vocommons/voaf#Vocabulary> .


###  Generated by the OWL API (version 4.2.8.20170104-2310) https://github.com/owlcs/owlapi
