@prefix : <https://w3id.org/rsp/vocals#> .
@prefix owl: <http://www.w3.org/2002/07/owl#> .
@prefix rdf: <http://www.w3.org/1999/02/22-rdf-syntax-ns#> .
@prefix xml: <http://www.w3.org/XML/1998/namespace> .
@prefix xsd: <http://www.w3.org/2001/XMLSchema#> .
@prefix dcat: <http://www.w3.org/ns/dcat#> .
@prefix foaf: <http://xmlns.com/foaf/0.1/> .
@prefix rdfs: <http://www.w3.org/2000/01/rdf-schema#> .

<https://w3id.org/rsp/vocals> a owl:Ontology ;
	owl:imports <http://www.w3.org/ns/dcat#> ;
	<http://purl.org/dc/elements/1.1/publisher> <http://aislab.hevs.ch/> ;
	<http://purl.org/dc/terms/creator> <http://streamreasoning.org/vois#RiccardoTommasini> ;
	rdfs:comment "This ontology aims to model RDF streams, their metadata, and access endpoints for publishing and consuming these streams"@en ;
	<http://purl.org/dc/terms/title> "VoCaLS: ontologie de representation de données et metadonnées de streams"@fr ;
	<http://purl.org/vocab/vann/preferredNamespaceUri> "https://w3id.org/rsp/vocals#"^^xsd:string ;
	<http://purl.org/dc/terms/creator> <http://w3id.org/people/jpcik/me> ;
	<http://purl.org/dc/terms/title> "VoCaLS: A Vocabulary and Catalog for Linked Streams"@en ;
	<http://purl.org/dc/terms/modified> "2017-12-10"^^xsd:date ;
	<http://purl.org/dc/terms/rights> "Copyright © 2017 Politecnico di Milano & HES-SO Valais-Wallis"^^xsd:string ;
	<http://purl.org/vocab/vann/preferredNamespacePrefix> "vocals"^^xsd:string ;
	<http://purl.org/dc/terms/title> "VoCaLS: Vocabulario y catálogo para Streams enlazados"@es ;
	<http://purl.org/dc/terms/issued> "2017-12-01"^^xsd:date ;
	rdfs:comment "Esta ontología has sido diseñada para representar Streams de datos en RDF, así como los endpoints a través de los cuales se puede acceder a los datos de estos streams;  y los meta datos correspondientes."@es ;
	<http://purl.org/dc/terms/license> <https://creativecommons.org/licenses/by/4.0/> ;
	<http://purl.org/dc/terms/publisher> <http://w3id.org/hes-so/aislab> ;
	<http://purl.org/dc/terms/description> "This ontology aims to model RDF streams, their metadata, and access endpoints for publishing and consuming these streams"@en ;
	<http://purl.org/dc/terms/creator> <http://streamreasoning.org/vois#YehiaAboSedira> ;
	<http://purl.org/dc/terms/description> "Esta ontología has sido diseñada para representar Streams de datos en RDF, así como los endpoints a través de los cuales se puede acceder a los datos de estos streams y los meta datos correspondientes."@es , "Cette ontologie a été conçue pour representer des données et meta-données de streams RDF, ainsi que leurs points d'accès."@fr ;
	rdfs:comment "Cette ontologie a été conçue pour representer des données et meta-données de streams RDF, ainsi que leurs points d'accès."@fr ;
	owl:versionInfo "0.1.1"^^xsd:string .
# 
# 
# #################################################################
# #
# #    Object Properties
# #
# #################################################################
# 
# 
# http://www.w3.org/ns/dcat#distribution

dcat:distribution a owl:ObjectProperty .
# 
# https://w3id.org/rsp/vocals#hasEndpoint

:hasEndpoint a owl:ObjectProperty ;
	rdfs:subPropertyOf dcat:distribution ;
	rdfs:domain :Stream ;
	rdfs:range :StreamEndpoint ;
	rdfs:comment "A relationship between a Stream and a StreamEndpoint. A stream may have several endpoints through which its contents can be accessible."@en ;
	rdfs:isDefinedBy <https://w3id.org/rsp/vocals#> ;
	rdfs:label "hasEndpoint"@en ;
	rdfs:seeAlso :Stream , :StreamEndpoint .
# 
# https://w3id.org/rsp/vocals#hasPartition

:hasPartition a owl:ObjectProperty ;
	rdfs:domain :Stream ;
	rdfs:range :StreamPartition ;
	rdfs:comment "A relationship between a Stream and a partition, or portion of elements streamed"@en ;
	rdfs:isDefinedBy <https://w3id.org/rsp/vocals#> ;
	rdfs:label "hasPartition"@en ;
	rdfs:seeAlso :Stream , :StreamPartition .
# 
# https://w3id.org/rsp/vocals#previous

:previous a owl:ObjectProperty ;
	rdfs:domain :StreamPartition ;
	rdfs:range :StreamPartition ;
	rdfs:comment "Relationship between a stream partition and the previous partition in the stream"@en ;
	rdfs:isDefinedBy <https://w3id.org/rsp/vocals#> ;
	rdfs:label "previous"@en ;
	rdfs:seeAlso :StreamPartition .
# 
# 
# 
# #################################################################
# #
# #    Classes
# #
# #################################################################
# 
# 
# http://purl.org/vocommons/voaf#Vocabulary

<http://purl.org/vocommons/voaf#Vocabulary> a owl:Class .
# 
# http://www.w3.org/ns/dcat#CatalogRecord

dcat:CatalogRecord a owl:Class .
# 
# http://www.w3.org/ns/dcat#Dataset

dcat:Dataset a owl:Class .
# 
# http://www.w3.org/ns/dcat#Distribution

dcat:Distribution a owl:Class .
# 
# http://xmlns.com/foaf/0.1/Document

foaf:Document a owl:Class .
# 
# https://w3id.org/rsp/vocals#RDFStream

:RDFStream a owl:Class ;
	rdfs:subClassOf :Stream ;
	rdfs:comment "A stream composed of RDF data elements, i.e. RDF graphs and/or triples."@en ;
	rdfs:isDefinedBy <https://w3id.org/rsp/vocals#> ;
	rdfs:label "RDFStream"@en ;
	rdfs:seeAlso :Stream .
# 
# https://w3id.org/rsp/vocals#Stream

:Stream a owl:Class ;
	rdfs:subClassOf dcat:Dataset ;
	rdfs:comment "A potentially infinite sequence of data elements. A stream may be findable and accesible on the Web."@en ;
	rdfs:isDefinedBy <https://w3id.org/rsp/vocals#> ;
	rdfs:label "Stream"@en ;
	rdfs:seeAlso :StreamDistribution .
# 
# https://w3id.org/rsp/vocals#StreamDescriptor

:StreamDescriptor a owl:Class ;
	rdfs:subClassOf dcat:CatalogRecord , foaf:Document ;
	rdfs:comment "A Stream Descriptor is a Web document that contains the description of a Stream."@en ;
	rdfs:isDefinedBy <https://w3id.org/rsp/vocals#> ;
	rdfs:label "StreamDescriptor"@en ;
	rdfs:seeAlso :Stream .
# 
# https://w3id.org/rsp/vocals#StreamDistribution

:StreamDistribution a owl:Class ;
	owl:equivalentClass :StreamEndpoint ;
	rdfs:subClassOf dcat:Distribution ;
	rdfs:comment "Represents a specific available form of a stream. Each stream might be available in different forms, these forms might represent different access points of the stream. Examples of distributions include a WebSocket endpoint, an HTTP endpoint, a Server-Sent Events endpoint, MQTT, etc."@en ;
	rdfs:isDefinedBy <https://w3id.org/rsp/vocals#> ;
	rdfs:label "StreamDistribution"@en ;
	rdfs:seeAlso :Stream .
# 
# https://w3id.org/rsp/vocals#StreamEndpoint

:StreamEndpoint a owl:Class ;
	rdfs:subClassOf dcat:Distribution ;
	rdfs:comment "Represents a specific available form of a stream. Each stream might be available in different forms, these forms might represent different access points of the stream. Examples of endpoints include a WebSocket endpoint, an HTTP endpoint, a Server-Sent Events endpoint, MQTT, etc."@en ;
	rdfs:isDefinedBy <https://w3id.org/rsp/vocals#> ;
	rdfs:label "StreamEndpoint"@en .
# 
# https://w3id.org/rsp/vocals#StreamPartition

:StreamPartition a owl:Class ;
	rdfs:subClassOf dcat:Dataset ;
	rdfs:comment "A portion of the time-varying data items of a Stream"@en ;
	rdfs:isDefinedBy <https://w3id.org/rsp/vocals#> ;
	rdfs:label "StreamPartition"@en ;
	rdfs:seeAlso :Stream .
# 
# 
# 
# #################################################################
# #
# #    Individuals
# #
# #################################################################
# 
# 
# https://w3id.org/rsp/vocals#

<https://w3id.org/rsp/vocals#> a owl:NamedIndividual , <http://purl.org/vocommons/voaf#Vocabulary> .
# 
# Generated by the OWL API (version 4.2.5.20160517-0735) https://github.com/owlcs/owlapi
